Hoare.v
@@ -1,5 +1,4 @@
-(** * Hoare: Hoare Logic *)
-
+(** * Hoare: Hoare Logic, Part I *)
 
 Require Export Imp.
 
@@ -90,7 +89,7 @@ Require Export Imp.
 
 Definition Assertion := state -> Prop.
 
-(** **** Exercise: 1 star, optional (assertions) *)
+(** **** Exercise: 1 star, optional (assertions)  *)
 Module ExAssertions.
 
 (** Paraphrase the following assertions in English. *)
@@ -110,6 +109,9 @@ Definition as6 : Assertion := fun st => False.
 End ExAssertions.
 (** [] *)
 
+(* ####################################################### *)
+(** ** Notation for Assertions *)
+
 (** This way of writing assertions can be a little bit heavy,
     for two reasons: (1) every single assertion that we ever write is
     going to begin with [fun st => ]; and (2) this state [st] is the
@@ -119,10 +121,10 @@ End ExAssertions.
     conventions: we'll drop the initial [fun st =>], and we'll write
     just [X] to mean [st X].  Thus, instead of writing *)
 (** 
-      fun st => (st Z) * (st Z) <= x /\
-                ~ ((S (st Z)) * (S (st Z)) <= x)
+      fun st => (st Z) * (st Z) <= m /\
+                ~ ((S (st Z)) * (S (st Z)) <= m)
     we'll write just
-         Z * Z <= x /\ ~((S Z) * (S Z) <= x).
+         Z * Z <= m /\ ~((S Z) * (S Z) <= m).
 *)
 
 (** Given two assertions [P] and [Q], we say that [P] _implies_ [Q],
@@ -183,23 +185,23 @@ Notation "{{ P }}  c  {{ Q }}" :=
     contexts.  The [Open Scope] tells Coq that this file is one such
     context.) *)
 
-(** **** Exercise: 1 star (triples) *)
+(** **** Exercise: 1 star, optional (triples)  *)
 (** Paraphrase the following Hoare triples in English.
    1) {{True}} c {{X = 5}}
 
-   2) {{X = x}} c {{X = x + 5)}}
+   2) {{X = m}} c {{X = m + 5)}}
 
    3) {{X <= Y}} c {{Y <= X}}
 
    4) {{True}} c {{False}}
 
-   5) {{X = x}} 
+   5) {{X = m}} 
       c
-      {{Y = real_fact x}}.
+      {{Y = real_fact m}}.
 
    6) {{True}} 
       c 
-      {{(Z * Z) <= x /\ ~ (((S Z) * (S Z)) <= x)}}
+      {{(Z * Z) <= m /\ ~ (((S Z) * (S Z)) <= m)}}
 
  *)
 
@@ -214,7 +216,7 @@ Notation "{{ P }}  c  {{ Q }}" :=
 
 
 
-(** **** Exercise: 1 star (valid_triples) *)
+(** **** Exercise: 1 star, optional (valid_triples)  *)
 (** Which of the following Hoare triples are _valid_ -- i.e., the
     claimed relation between [P], [c], and [Q] is true?
    1) {{True}} X ::= 5 {{X = 5}}
@@ -411,7 +413,7 @@ Example assn_sub_example :
 Proof.
   apply hoare_asgn.  Qed.
 
-(** **** Exercise: 2 stars (hoare_asgn_examples) *)
+(** **** Exercise: 2 stars (hoare_asgn_examples)  *)
 (** Translate these informal Hoare triples...
     1) {{ (X <= 5) [X |-> X + 1] }}
        X ::= X + 1
@@ -420,12 +422,13 @@ Proof.
     2) {{ (0 <= X /\ X <= 5) [X |-> 3] }}
        X ::= 3
        {{ 0 <= X /\ X <= 5 }}
-   ...into formal statements and use [hoare_asgn] to prove them. *)
+   ...into formal statements [assn_sub_ex1, assn_sub_ex2] 
+   and use [hoare_asgn] to prove them. *)
 
 (* FILL IN HERE *)
 (** [] *)
 
-(** **** Exercise: 2 stars (hoare_asgn_wrong) *)
+(** **** Exercise: 2 stars (hoare_asgn_wrong)  *)
 (** The assignment rule looks backward to almost everyone the first
     time they see it.  If it still seems backward to you, it may help
     to think a little about alternative "forward" rules.  Here is a
@@ -440,15 +443,15 @@ Proof.
 (* FILL IN HERE *)
 (** [] *)
 
-(** **** Exercise: 3 stars, optional (hoare_asgn_fwd) *)
-(** However, using an auxiliary variable [x] to remember the original
+(** **** Exercise: 3 stars, advanced (hoare_asgn_fwd)  *)
+(** However, using an auxiliary variable [m] to remember the original
     value of [X] we can define a Hoare rule for assignment that does,
     intuitively, "work forwards" rather than backwards.
   ------------------------------------------ (hoare_asgn_fwd)
-  {{fun st => Q st /\ st X = x}}
+  {{fun st => P st /\ st X = m}}
     X ::= a
-  {{fun st => Q st' /\ st X = aeval st' a }}
-  (where st' = update st X x)
+  {{fun st => P st' /\ st X = aeval st' a }}
+  (where st' = update st X m)
     Note that we use the original value of [X] to reconstruct the
     state [st'] before the assignment took place. Prove that this rule
     is correct (the first hypothesis is the functional extensionality
@@ -457,13 +460,39 @@ Proof.
 *)
 
 Theorem hoare_asgn_fwd :
-  (forall {X Y: Type} {f g : X -> Y}, (forall (x: X), f x = g x) ->  f = g) ->
-  forall x a Q,
-  {{fun st => Q st /\ st X = x}}
+  (forall {X Y: Type} {f g : X -> Y},
+     (forall (x: X), f x = g x) ->  f = g) ->
+  forall m a P,
+  {{fun st => P st /\ st X = m}}
     X ::= a
-  {{fun st => Q (update st X x) /\ st X = aeval (update st X x) a }}.
+  {{fun st => P (update st X m) /\ st X = aeval (update st X m) a }}.
 Proof.
-  intros functional_extensionality v a Q.
+  intros functional_extensionality m a P.
+  (* FILL IN HERE *) Admitted.
+(** [] *)
+
+(** **** Exercise: 2 stars, advanced (hoare_asgn_fwd_exists)  *)
+(** Another way to define a forward rule for assignment is to
+    existentially quantify over the previous value of the assigned
+    variable.
+  ------------------------------------------ (hoare_asgn_fwd_exists)
+  {{fun st => P st}}
+    X ::= a
+  {{fun st => exists m, P (update st X m) /\
+                 st X = aeval (update st X m) a }}
+*)
+(* This rule was proposed by Nick Giannarakis and Zoe Paraskevopoulou. *)
+
+Theorem hoare_asgn_fwd_exists :
+  (forall {X Y: Type} {f g : X -> Y},
+     (forall (x: X), f x = g x) ->  f = g) ->
+  forall a P,
+  {{fun st => P st}}
+    X ::= a
+  {{fun st => exists m, P (update st X m) /\
+                st X = aeval (update st X m) a }}.
+Proof.
+  intros functional_extensionality a P.
   (* FILL IN HERE *) Admitted.
 (** [] *)
 
@@ -529,7 +558,7 @@ Proof.
   assumption. assumption. Qed.
 
 (** For example, we might use the first consequence rule like this:
-                {{ True }} =>
+                {{ True }} ->>
                 {{ 1 = 1 }} 
     X ::= 1
                 {{ X = 1 }}
@@ -593,15 +622,15 @@ Example hoare_asgn_example1' :
 Proof.
   eapply hoare_consequence_pre.
   apply hoare_asgn.
-  intros st H. reflexivity.  Qed.
+  intros st H.  reflexivity.  Qed.
 
-(** In general, [eapply H] tactic works just like [apply H]
-    except that, instead of failing if unifying the goal with the
-    conclusion of [H] does not determine how to instantiate all
-    of the variables appearing in the premises of [H], [eapply H]
-    will replace these variables with _existential variables_
-    (written [?nnn]) as placeholders for expressions that will be
-    determined (by further unification) later in the proof. *)
+(** In general, [eapply H] tactic works just like [apply H] except
+    that, instead of failing if unifying the goal with the conclusion
+    of [H] does not determine how to instantiate all of the variables
+    appearing in the premises of [H], [eapply H] will replace these
+    variables with so-called _existential variables_ (written [?nnn])
+    as placeholders for expressions that will be determined (by
+    further unification) later in the proof. *)
 
 (** In order for [Qed] to succeed, all existential variables need to
     be determined by the end of the proof. Otherwise Coq
@@ -623,6 +652,10 @@ Proof.
              Q : nat -> Prop
              HP : forall x y : nat, P x y
              HQ : forall x y : nat, P x y -> Q x |- nat] 
+  
+     (dependent evars: ?171 open,)
+
+     You can use Grab Existential Variables.
    Trying to finish the proof with [Qed] gives an error:
 <<
     Error: Attempt to save a proof with existential variables still
@@ -642,7 +675,6 @@ Lemma silly2 :
   Q 42.
 Proof.
   intros P Q HP HQ. eapply HQ. destruct HP as [y HP'].
-
 (** Doing [apply HP'] above fails with the following error:
      Error: Impossible to unify "?175" with "y".
     In this case there is an easy fix:
@@ -677,12 +709,14 @@ Proof.
   intros P Q HP HQ. destruct HP as [y HP']. eapply HQ. eassumption.
 Qed.
 
-(** **** Exercise: 2 stars (hoare_asgn_examples_2) *)
+    
+
+(** **** Exercise: 2 stars (hoare_asgn_examples_2)  *)
 (** Translate these informal Hoare triples...
        {{ X + 1 <= 5 }}  X ::= X + 1  {{ X <= 5 }}
        {{ 0 <= 3 /\ 3 <= 5 }}  X ::= 3  {{ 0 <= X /\ X <= 5 }}
-   ...into formal statements and use [hoare_asgn] and
-   [hoare_consequence_pre] to prove them. *)
+   ...into formal statements [assn_sub_ex1', assn_sub_ex2'] and 
+   use [hoare_asgn] and [hoare_consequence_pre] to prove them. *)
 
 (* FILL IN HERE *)
 (** [] *)
@@ -713,13 +747,13 @@ Proof.
         {{ P }} c1 {{ Q }} 
         {{ Q }} c2 {{ R }}
        ---------------------  (hoare_seq)
-       {{ P }} c1;c2 {{ R }}
+       {{ P }} c1;;c2 {{ R }}
 *)
 
 Theorem hoare_seq : forall P Q R c1 c2,
      {{Q}} c2 {{R}} ->
      {{P}} c1 {{Q}} ->
-     {{P}} c1;c2 {{R}}.
+     {{P}} c1;;c2 {{R}}.
 Proof.
   intros P Q R c1 c2 H1 H2 st st' H12 Pre.
   inversion H12; subst.
@@ -738,7 +772,7 @@ Proof.
     rule is as a "decorated program" where the intermediate assertion
     [Q] is written between [c1] and [c2]:
       {{ a = n }}
-    X ::= a;
+    X ::= a;;
       {{ X = n }}      <---- decoration for Q
     SKIP
       {{ X = n }}
@@ -746,7 +780,7 @@ Proof.
 
 Example hoare_asgn_example3 : forall a n,
   {{fun st => aeval st a = n}} 
-  (X ::= a; SKIP) 
+  (X ::= a;; SKIP) 
   {{fun st => st X = n}}.
 Proof.
   intros a n. eapply hoare_seq.
@@ -760,11 +794,11 @@ Proof.
     [hoare_consequence_pre] in conjunction with the [eapply] tactic,
     as done above. *)
 
-(** **** Exercise: 2 stars (hoare_asgn_example4) *)
+(** **** Exercise: 2 stars (hoare_asgn_example4)  *)
 (** Translate this "decorated program" into a formal proof:
                    {{ True }} ->>
                    {{ 1 = 1 }}
-    X ::= 1;
+    X ::= 1;;
                    {{ X = 1 }} ->>
                    {{ X = 1 /\ 2 = 2 }}
     Y ::= 2
@@ -772,28 +806,13 @@ Proof.
 *)
 
 Example hoare_asgn_example4 :
-  {{fun st => True}} (X ::= (ANum 1); Y ::= (ANum 2)) 
+  {{fun st => True}} (X ::= (ANum 1);; Y ::= (ANum 2)) 
   {{fun st => st X = 1 /\ st Y = 2}}.
 Proof.
-  apply hoare_seq with (Q := fun st => st X = 1).
-  eapply hoare_consequence_pre. apply hoare_asgn.
-  intros st H. split. assumption. reflexivity.
-  eapply hoare_consequence_pre. apply hoare_asgn.
-  intros st H. reflexivity.
-Qed.
-  
-(*
-  intros st H.
-  split.
-  inversion H0; subst.
-  inversion H7; subst.
-  inversion H4; subst. reflexivity.
-  inversion H0; subst.
-  inversion H7; subst. reflexivity.
-Qed.
-*)
+  (* FILL IN HERE *) Admitted.
+(** [] *)
 
-(** **** Exercise: 3 stars (swap_exercise) *)
+(** **** Exercise: 3 stars (swap_exercise)  *)
 (** Write an Imp program [c] that swaps the values of [X] and [Y]
     and show (in Coq) that it satisfies the following
     specification:
@@ -811,11 +830,11 @@ Proof.
   (* FILL IN HERE *) Admitted.
 (** [] *)
 
-(** **** Exercise: 3 stars, optional (hoarestate1) *)
+(** **** Exercise: 3 stars (hoarestate1)  *)
 (** Explain why the following proposition can't be proven:
       forall (a : aexp) (n : nat),
          {{fun st => aeval st a = n}}
-         (X ::= (ANum 3); Y ::= a)
+         (X ::= (ANum 3);; Y ::= a)
          {{fun st => st Y = n}}.
 *)
 
@@ -842,15 +861,16 @@ Proof.
      FI
      {{ X <= Y }}
    since the rule tells us nothing about the state in which the
-   assignments take place in the "then" and "else" branches.
+   assignments take place in the "then" and "else" branches. *)
    
-   But we can actually say something more precise.  In the "then"
-   branch, we know that the boolean expression [b] evaluates to
+(** But we can actually say something more precise.  In the
+   "then" branch, we know that the boolean expression [b] evaluates to
    [true], and in the "else" branch, we know it evaluates to [false].
    Making this information available in the premises of the rule gives
    us more information to work with when reasoning about the behavior
    of [c1] and [c2] (i.e., the reasons why they establish the
-   postcondition [Q]).
+   postcondition [Q]). *)
+(**
               {{P /\  b}} c1 {{Q}}
               {{P /\ ~b}} c2 {{Q}}
       ------------------------------------  (hoare_if)
@@ -904,6 +924,59 @@ Proof.
       split. assumption.
              apply bexp_eval_false. assumption. Qed.
 
+
+(* ####################################################### *) 
+
+(** * Hoare Logic: So Far *)
+
+(** 
+Idea: create a _domain specific logic_ for reasoning about properties of Imp programs.
+
+- This hides the low-level details of the semantics of the program
+- Leads to a compositional reasoning process
+
+
+The basic structure is given by _Hoare triples_ of the form:
+  {{P}} c {{Q}}
+]] 
+
+- [P] and [Q] are predicates about the state of the Imp program
+- "If command [c] is started in a state satisfying assertion
+        [P], and if [c] eventually terminates in some final state,
+        then this final state will satisfy the assertion [Q]."
+
+*)
+
+
+(** ** Hoare Logic Rules (so far) *)
+
+(**
+             ------------------------------ (hoare_asgn)
+             {{Q [X |-> a]}} X::=a {{Q}}
+
+             --------------------  (hoare_skip)
+             {{ P }} SKIP {{ P }}
+
+               {{ P }} c1 {{ Q }} 
+               {{ Q }} c2 {{ R }}
+              ---------------------  (hoare_seq)
+              {{ P }} c1;;c2 {{ R }}
+
+              {{P /\  b}} c1 {{Q}}
+              {{P /\ ~b}} c2 {{Q}}
+      ------------------------------------  (hoare_if)
+      {{P}} IFB b THEN c1 ELSE c2 FI {{Q}} 
+
+
+                {{P'}} c {{Q'}}
+                   P ->> P'
+                   Q' ->> Q
+         -----------------------------   (hoare_consequence)
+                {{P}} c {{Q}}
+*)
+
+
+(** *** Example *)
 (** Here is a formal proof that the program we used to motivate the
     rule satisfies the specification we gave. *)
 
@@ -915,12 +988,13 @@ Example if_example :
   FI
     {{fun st => st X <= st Y}}.
 Proof.
+  (* WORKED IN CLASS *)
   apply hoare_if.
   Case "Then".
     eapply hoare_consequence_pre. apply hoare_asgn.
     unfold bassn, assn_sub, update, assert_implies.
     simpl. intros st [_ H].
-    symmetry in H; apply beq_nat_eq in H.
+    apply beq_nat_true in H.
     rewrite H. omega.
   Case "Else".
     eapply hoare_consequence_pre. apply hoare_asgn.
@@ -928,7 +1002,7 @@ Proof.
     simpl; intros st _. omega.
 Qed.
 
-(** **** Exercise: 2 stars (if_minus_plus) *)
+(** **** Exercise: 2 stars (if_minus_plus)  *)
 (** Prove the following hoare triple using [hoare_if]: *)
 
 Theorem if_minus_plus :
@@ -939,23 +1013,12 @@ Theorem if_minus_plus :
   FI
   {{fun st => st Y = st X + st Z}}. 
 Proof.
-  apply hoare_if.
-  Case "true".
-    eapply hoare_consequence_pre. apply hoare_asgn.
-    unfold bassn. unfold assn_sub. unfold assert_implies.
-    simpl. intros. inversion H. unfold update. simpl.
-    apply ble_nat_true in H1. omega.
-  Case "false".
-    eapply hoare_consequence_pre. apply hoare_asgn.
-    unfold bassn. unfold assn_sub. unfold assert_implies.
-    simpl. intros. inversion H. unfold update; simpl.
-    reflexivity.
-Qed.
+  (* FILL IN HERE *) Admitted.
 
 (* ####################################################### *)
 (** *** Exercise: One-sided conditionals *)
 
-(** **** Exercise: 4 stars (if1_hoare) *)
+(** **** Exercise: 4 stars (if1_hoare)  *)
 
 (** In this exercise we consider extending Imp with "one-sided
     conditionals" of the form [IF1 b THEN c FI]. Here [b] is a
@@ -989,7 +1052,7 @@ Tactic Notation "com_cases" tactic(first) ident(c) :=
 
 Notation "'SKIP'" := 
   CSkip.
-Notation "c1 ; c2" := 
+Notation "c1 ;; c2" := 
   (CSeq c1 c2) (at level 80, right associativity).
 Notation "X '::=' a" := 
   (CAss X a) (at level 60).
@@ -1011,7 +1074,7 @@ Inductive ceval : com -> state -> state -> Prop :=
   | E_Ass : forall (st : state) (a1 : aexp) (n : nat) (X : id),
             aeval st a1 = n -> (X ::= a1) / st || update st X n
   | E_Seq : forall (c1 c2 : com) (st st' st'' : state),
-            c1 / st || st' -> c2 / st' || st'' -> (c1 ; c2) / st || st''
+            c1 / st || st' -> c2 / st' || st'' -> (c1 ;; c2) / st || st''
   | E_IfTrue : forall (st st' : state) (b1 : bexp) (c1 c2 : com),
                beval st b1 = true ->
                c1 / st || st' -> (IFB b1 THEN c1 ELSE c2 FI) / st || st'
@@ -1056,8 +1119,8 @@ Notation "{{ P }}  c  {{ Q }}" := (hoare_triple P c Q)
 
 (* FILL IN HERE *)
 
-(** For full credit, prove formally that your rule is precise enough
-    to show the following valid Hoare triple:
+(** For full credit, prove formally [hoare_if1_good] that your rule is 
+    precise enough to show the following valid Hoare triple:
   {{ X + Y = Z }}
   IF1 Y <> 0 THEN
     X ::= X + Y
@@ -1084,24 +1147,37 @@ End If1.
 (* ####################################################### *)
 (** *** Loops *)
 
-(** Finally, we need a rule for reasoning about while loops.  Suppose
-    we have a loop
+(** Finally, we need a rule for reasoning about while loops. *)
+
+(** Suppose we have a loop
       WHILE b DO c END
     and we want to find a pre-condition [P] and a post-condition
     [Q] such that
       {{P}} WHILE b DO c END {{Q}} 
     is a valid triple. *)
 
+(** *** *)
+
 (** First of all, let's think about the case where [b] is false at the
     beginning -- i.e., let's assume that the loop body never executes
     at all.  In this case, the loop behaves like [SKIP], so we might
-    be tempted to write
+    be tempted to write: *)
+
+(**
       {{P}} WHILE b DO c END {{P}}.
+*)
+
+(** 
     But, as we remarked above for the conditional, we know a
     little more at the end -- not just [P], but also the fact
     that [b] is false in the current state.  So we can enrich the
     postcondition a little:
+*)
+(** 
       {{P}} WHILE b DO c END {{P /\ ~b}}
+*)
+
+(** 
     What about the case where the loop body _does_ get executed?
     In order to ensure that [P] holds when the loop finally
     exits, we certainly need to make sure that the command [c]
@@ -1111,24 +1187,26 @@ End If1.
     re-establishes [P] when it finishes, we can always assume
     that [P] holds at the beginning of [c].  This leads us to the
     following rule:
+*)
+(** 
                    {{P}} c {{P}}
         -----------------------------------  
         {{P}} WHILE b DO c END {{P /\ ~b}}
-    The proposition [P] is called an _invariant_.
-
+*)
+(** 
     This is almost the rule we want, but again it can be improved a
     little: at the beginning of the loop body, we know not only that
     [P] holds, but also that the guard [b] is true in the current
     state.  This gives us a little more information to use in
     reasoning about [c] (showing that it establishes the invariant by
     the time it finishes).  This gives us the final version of the rule:
+*)
+(**
                {{P /\ b}} c {{P}}
         -----------------------------------  (hoare_while)
         {{P}} WHILE b DO c END {{P /\ ~b}}
+    The proposition [P] is called an _invariant_ of the loop.
 *)
-
-
-
 
 Lemma hoare_while : forall P b c,
   {{fun st => P st /\ bassn b st}} c {{P}} ->
@@ -1136,20 +1214,38 @@ Lemma hoare_while : forall P b c,
 Proof.
   intros P b c Hhoare st st' He HP.
   (* Like we've seen before, we need to reason by induction 
-     on He, because, in the "keep looping" case, its hypotheses 
-     talk about the whole loop instead of just c *)
-  remember (WHILE b DO c END) as wcom.
+     on [He], because, in the "keep looping" case, its hypotheses 
+     talk about the whole loop instead of just [c]. *)
+  remember (WHILE b DO c END) as wcom eqn:Heqwcom.
   ceval_cases (induction He) Case;
-    try (inversion Heqwcom); subst.
-
+    try (inversion Heqwcom); subst; clear Heqwcom.
   Case "E_WhileEnd".
     split. assumption. apply bexp_eval_false. assumption.
-
   Case "E_WhileLoop".
     apply IHHe2. reflexivity.
     apply (Hhoare st st'). assumption.
       split. assumption. apply bexp_eval_true. assumption.
 Qed.
+
+(**
+    One subtlety in the terminology is that calling some assertion [P]
+    a "loop invariant" doesn't just mean that it is preserved by the
+    body of the loop in question (i.e., [{{P}} c {{P}}], where [c] is
+    the loop body), but rather that [P] _together with the fact that
+    the loop's guard is true_ is a sufficient precondition for [c] to
+    ensure [P] as a postcondition.
+
+    This is a slightly (but significantly) weaker requirement.  For
+    example, if [P] is the assertion [X = 0], then [P] _is_ an
+    invariant of the loop
+    WHILE X = 2 DO X := 1 END
+    although it is clearly _not_ preserved by the body of the
+    loop.
+*)
+
+
+
+
 
 Example while_example :
     {{fun st => st X <= 3}}
@@ -1164,17 +1260,24 @@ Proof.
   unfold bassn, assn_sub, assert_implies, update. simpl.
     intros st [H1 H2]. apply ble_nat_true in H2. omega.
   unfold bassn, assert_implies. intros st [Hle Hb]. 
-    simpl in Hb. remember (ble_nat (st X) 2) as le. destruct le. 
+    simpl in Hb. destruct (ble_nat (st X) 2) eqn : Heqle. 
     apply ex_falso_quodlibet. apply Hb; reflexivity.  
-    symmetry in Heqle. apply ble_nat_false in Heqle. omega. 
+    apply ble_nat_false in Heqle. omega. 
 Qed.
 
-(** We can also use the while rule to prove the following Hoare
-    triple, which may seem surprising at first... *)
+
+
+
+
+
+(** *** *)
+(** We can use the while rule to prove the following Hoare triple,
+    which may seem surprising at first... *)
 
 Theorem always_loop_hoare : forall P Q,
   {{P}} WHILE BTrue DO SKIP END {{Q}}.
 Proof.
+  (* WORKED IN CLASS *)
   intros P Q.
   apply hoare_consequence_pre with (P' := fun st : state => True).
   eapply hoare_consequence_post.
@@ -1187,35 +1290,24 @@ Proof.
   Case "Precondition implies invariant".
     intros st H. constructor.  Qed.
 
-(** Actually, this result shouldn't be surprising.  If we look back at
-    the definition of [hoare_triple], we can see that it asserts
-    something meaningful _only_ when the command terminates. *)
+(** Of course, this result is not surprising if we remember that
+    the definition of [hoare_triple] asserts that the postcondition
+    must hold _only_ when the command terminates.  If the command
+    doesn't terminate, we can prove anything we like about the
+    post-condition. *)
 
-Print hoare_triple.
-
-(** If the command doesn't terminate, we can prove anything we like
-    about the post-condition.  Here's a more direct proof of the same
-    fact: *)
-
-Theorem always_loop_hoare' : forall P Q,
-  {{P}} WHILE BTrue DO SKIP END {{Q}}.
-Proof.  
-  unfold hoare_triple. intros P Q st st' contra.
-  apply loop_never_stops in contra.  inversion contra. 
-Qed.
-
-(** Hoare rules that only talk about terminating commands are often
-    said to describe a logic of "partial" correctness.  It is also
-    possible to give Hoare rules for "total" correctness, which build
-    in the fact that the commands terminate. However, in this course
-    we will focus only on partial correctness. *)
+(** Hoare rules that only talk about terminating commands are
+    often said to describe a logic of "partial" correctness.  It is
+    also possible to give Hoare rules for "total" correctness, which
+    build in the fact that the commands terminate. However, in this
+    course we will only talk about partial correctness. *)
 
 (* ####################################################### *)
 (** *** Exercise: [REPEAT] *)
 
 Module RepeatExercise.
 
-(** **** Exercise: 4 stars (hoare_repeat) *)
+(** **** Exercise: 4 stars, advanced (hoare_repeat)  *)
 (** In this exercise, we'll add a new command to our language of
     commands: [REPEAT] c [UNTIL] a [END]. You will write the
     evaluation rule for [repeat] and add a new Hoare rule to
@@ -1242,7 +1334,7 @@ Tactic Notation "com_cases" tactic(first) ident(c) :=
 
 Notation "'SKIP'" := 
   CSkip.
-Notation "c1 ; c2" := 
+Notation "c1 ;; c2" := 
   (CSeq c1 c2) (at level 80, right associativity).
 Notation "X '::=' a" := 
   (CAsgn X a) (at level 60).
@@ -1268,7 +1360,7 @@ Inductive ceval : state -> com -> state -> Prop :=
   | E_Seq : forall c1 c2 st st' st'',
       ceval st c1 st' ->
       ceval st' c2 st'' ->
-      ceval st (c1 ; c2) st''
+      ceval st (c1 ;; c2) st''
   | E_IfTrue : forall st st' b1 c1 c2,
       beval st b1 = true ->
       ceval st c1 st' ->
@@ -1315,7 +1407,7 @@ Notation "{{ P }}  c  {{ Q }}" :=
 
 Definition ex1_repeat :=
   REPEAT
-    X ::= ANum 1;
+    X ::= ANum 1;;
     Y ::= APlus (AId Y) (ANum 1)
   UNTIL (BEq (AId X) (ANum 1)) END.
 
@@ -1332,10 +1424,10 @@ Proof.
 (* FILL IN HERE *)
 
 (** For full credit, make sure (informally) that your rule can be used
-    to prove the following _valid_ Hoare triple:
+    to prove the following valid Hoare triple:
   {{ X > 0 }}
   REPEAT
-    Y ::= X;
+    Y ::= X;;
     X ::= X - 1
   UNTIL X = 0 END
   {{ X = 0 /\ Y > 0 }}
@@ -1348,7 +1440,7 @@ End RepeatExercise.
 (* ####################################################### *)
 (** ** Exercise: [HAVOC] *)
 
-(** **** Exercise: 3 stars (himp_hoare) *)
+(** **** Exercise: 3 stars (himp_hoare)  *)
 
 (** In this exercise, we will derive proof rules for the [HAVOC] command
     which we studied in the last chapter. First, we enclose this work
@@ -1374,7 +1466,7 @@ Notation "'SKIP'" :=
   CSkip.
 Notation "X '::=' a" :=
   (CAsgn X a) (at level 60).
-Notation "c1 ; c2" :=
+Notation "c1 ;; c2" :=
   (CSeq c1 c2) (at level 80, right associativity).
 Notation "'WHILE' b 'DO' c 'END'" :=
   (CWhile b c) (at level 80, right associativity).
@@ -1389,7 +1481,7 @@ Inductive ceval : com -> state -> state -> Prop :=
   | E_Ass : forall (st : state) (a1 : aexp) (n : nat) (X : id),
             aeval st a1 = n -> (X ::= a1) / st || update st X n
   | E_Seq : forall (c1 c2 : com) (st st' st'' : state),
-            c1 / st || st' -> c2 / st' || st'' -> (c1 ; c2) / st || st''
+            c1 / st || st' -> c2 / st' || st'' -> (c1 ;; c2) / st || st''
   | E_IfTrue : forall (st st' : state) (b1 : bexp) (c1 c2 : com),
                beval st b1 = true ->
                c1 / st || st' -> (IFB b1 THEN c1 ELSE c2 FI) / st || st'
@@ -1444,7 +1536,7 @@ End Himp.
 
 
 (* ####################################################### *)
-(** * Review of Hoare Logic *)
+(** ** Complete List of Hoare Logic Rules *)
 
 (** Above, we've introduced Hoare Logic as a tool to reasoning
     about Imp programs. In the reminder of this chapter we will
@@ -1461,7 +1553,7 @@ End Himp.
                {{ P }} c1 {{ Q }} 
                {{ Q }} c2 {{ R }}
               ---------------------  (hoare_seq)
-              {{ P }} c1;c2 {{ R }}
+              {{ P }} c1;;c2 {{ R }}
 
               {{P /\  b}} c1 {{Q}}
               {{P /\ ~b}} c2 {{Q}}
@@ -1477,1361 +1569,9 @@ End Himp.
                    Q' ->> Q
          -----------------------------   (hoare_consequence)
                 {{P}} c {{Q}}
-    Next we'll see how these rules are used to prove that programs
-    satisfy specifications of their behavior.
+    In the next chapter, we'll see how these rules are used to prove
+    that programs satisfy specifications of their behavior.
 *)
 
-
-(* ####################################################### *)
-(** * Decorated Programs *)
-
-(** The beauty of Hoare Logic is that it is _compositional_ --
-    the structure of proofs exactly follows the structure of programs.
-    This suggests that we can record the essential ideas of a proof
-    informally (leaving out some low-level calculational details) by
-    decorating programs with appropriate assertions around each
-    statement.  Such a _decorated program_ carries with it
-    an (informal) proof of its own correctness. *)
-
-(** For example, here is a complete decorated program: *)
-(**
-      {{ True }} ->>
-      {{ x = x }}
-    X ::= x; 
-      {{ X = x }} ->> 
-      {{ X = x /\ z = z }}
-    Z ::= z;              
-      {{ X = x /\ Z = z }} ->>
-      {{ Z - X = z - x }}
-    WHILE X <> 0 DO
-        {{ Z - X = z - x /\ X <> 0 }} ->>
-        {{ (Z - 1) - (X - 1) = z - x }}
-      Z ::= Z - 1;               
-        {{ Z - (X - 1) = z - x }}
-      X ::= X - 1 
-        {{ Z - X = z - x }} 
-    END;
-      {{ Z - X = z - x /\ ~ (X <> 0) }} ->>
-      {{ Z = z - x }} ->>
-      {{ Z + 1 = z - x + 1 }}
-    Z ::= Z + 1
-      {{ Z = z - x + 1 }}
-*)
-
-(** Concretely, a decorated program consists of the program text
-    interleaved with assertions.  To check that a decorated program
-    represents a valid proof, we check that each individual command is
-    _locally_ consistent with its accompanying assertions in the
-    following sense: *)
-
-(** 
-    - [SKIP] is locally consistent if its precondition and
-      postcondition are the same:
-          {{ P }} 
-          SKIP
-          {{ P }} 
-    - The sequential composition of commands [c1] and [c2] is locally
-      consistent (with respect to assertions [P] and [R]) if [c1] is
-      locally consistent (with respect to [P] and [Q]) and [c2] is
-      locally consistent (with respect to [Q] and [R]):
-          {{ P }} 
-          c1;
-          {{ Q }} 
-          c2
-          {{ R }}
-
-    - An assignment is locally consistent if its precondition is
-      the appropriate substitution of its postcondition:
-          {{ P where a is substituted for X }}  
-          X ::= a  
-          {{ P }}
-    - A conditional is locally consistent (with respect to assertions
-      [P] and [Q]) if the assertions at the top of its "then" and
-      "else" branches are exactly [P /\ b] and [P /\ ~b] and if its "then"
-      branch is locally consistent (with respect to [P /\ b] and [Q])
-      and its "else" branch is locally consistent (with respect to
-      [P /\ ~b] and [Q]):
-          {{ P }} 
-          IFB b THEN
-            {{ P /\ b }} 
-            c1 
-            {{ Q }}
-          ELSE
-            {{ P /\ ~b }} 
-            c2
-            {{ Q }}
-          FI
-          {{ Q }}
-
-    - A while loop with precondition [P] is locally consistent if its
-      postcondition is [P /\ ~b] and if the pre- and postconditions of
-      its body are exactly [P /\ b] and [P]:
-          {{ P }} 
-          WHILE b DO
-            {{ P /\ b }} 
-            c1 
-            {{ P }}
-          END
-          {{ P /\ ~b }} 
-
-    - A pair of assertions separated by [->>] is locally consistent if
-      the first implies the second (in all states):
-          {{ P }} ->>
-          {{ P' }} 
-
-      This corresponds to the application of [hoare_consequence] and
-      is the only place in a decorated program where checking if
-      decorations are correct is not fully mechanical and syntactic,
-      but involves logical and/or arithmetic reasoning.
-*)
-
-(** We have seen above how _verifying_ the correctness of a given
-    proof involves checking that every single command is locally
-    consistent with the accompanying assertions.  If we are instead
-    interested in _finding_ a proof for a given specification we need
-    to discover the right assertions. This can be done in an almost
-    automatic way, with the exception of finding loop invariants,
-    which is the subject of in the next section.  In the reminder of
-    this section we explain in detail how to construct decorations for
-    several simple programs that don't involve non-trivial loop
-    invariants. *)
-
-(* ####################################################### *)
-(** ** Example: Swapping Using Addition and Subtraction *)
-
-(** Here is a program that swaps the values of two variables using
-    addition and subtraction.
-  X ::= X + Y;
-  Y ::= X - Y;
-  X ::= X - Y
-    We can prove using decorations that this program is correct --
-    i.e., it always swaps the values of variables [X] and [Y].
- (1)     {{ X = x /\ Y = y }} ->>
- (2)     {{ (X + Y) - ((X + Y) - Y) = y /\ (X + Y) - Y = x }}
-        X ::= X + Y;
- (3)     {{ X - (X - Y) = y /\ X - Y = x }}
-        Y ::= X - Y;
- (4)     {{ X - Y = y /\ Y = x }}
-        X ::= X - Y
- (5)     {{ X = y /\ Y = x }}
-    The decorations were constructed as follows:
-      - We begin with the undecorated program (the unnumbered lines).
-      - We then add the specification -- i.e., the outer
-        precondition (1) and postcondition (5). In the precondition we
-        use auxiliary variables (parameters) [x] and [y] to remember
-        the initial values of variables [X] and respectively [Y], so
-        that we can refer to them in the postcondition (5).
-      - We work backwards mechanically starting from (5) all the way
-        to (2). At each step, we obtain the precondition of the
-        assignment from its postcondition by substituting the assigned
-        variable with the right-hand-side of the assignment. For
-        instance, we obtain (4) by substituting [X] with [X - Y]
-        in (5), and (3) by substituting [Y] with [X - Y] in (4).
-      - Finally, we verify that (1) logically implies (2) -- i.e.,
-        that the step from (1) to (2) is a valid use of the law of
-        consequence. For this we substitute [X] by [x] and [Y] by [y]
-        and calculate as follows:
-            (x + y) - ((x + y) - y) = y /\ (x + y) - y = x
-            (x + y) - x = y /\ x = x
-            y = y /\ x = x
-
-    (Note that, since we are working with natural numbers, not
-    fixed-size machine integers, we don't need to worry about the
-    possibility of arithmetic overflow anywhere in this argument.)
-*)
-
-(* ####################################################### *)
-(** ** Example: Simple Conditionals *)
-
-(** Here is a simple decorated program using conditionals:
- (1)     {{True}}
-       IFB X <= Y THEN
- (2)       {{True /\ X <= Y}} ->>
- (3)       {{(Y - X) + X = Y \/ (Y - X) + Y = X}}
-         Z ::= AMinus (AId Y) (AId X)
- (4)       {{Z + X = Y \/ Z + Y = X}} 
-       ELSE
- (5)       {{True /\ ~(X <= Y) }} ->>
- (6)       {{(X - Y) + X = Y \/ (X - Y) + Y = X}}
-         Z ::= AMinus (AId X) (AId Y)
- (7)       {{Z + X = Y \/ Z + Y = X}}
-       FI
- (8)     {{Z + X = Y \/ Z + Y = X}}
-
-These decorations were constructed as follows:
-  - We start with the outer precondition (1) and postcondition (8).
-  - We follow the format dictated by the [hoare_if] rule and copy the
-    postcondition (8) to (4) and (7). We conjoin the precondition (1)
-    with the guard of the conditional to obtain (2). We conjoin (1)
-    with the negated guard of the conditional to obtain (5).
-  - In order to use the assignment rule and obtain (3), we substitute
-    [Z] by [Y - X] in (4). To obtain (6) we substitute [Z] by [X - Y]
-    in (7).
-  - Finally, we verify that (2) implies (3) and (5) implies (6). Both
-    of these implications crucially depend on the ordering of [X] and
-    [Y] obtained from the guard. For instance, knowing that [X <= Y]
-    ensures that subtracting [X] from [Y] and then adding back [X]
-    produces [Y], as required by the first disjunct of (3). Similarly,
-    knowing that [~(X <= Y)] ensures that subtracting [Y] from [X] and
-    then adding back [Y] produces [X], as needed by the second
-    disjunct of (6). Note that [n - m + m = n] does _not_ hold for
-    arbitrary natural numbers [n] and [m] (for example, [3 - 5 + 5 =
-    5]). *)
-
-(** **** Exercise: 2 stars (if_minus_plus_reloaded) *)
-(** Fill in valid decorations for the following program:
-   {{ True }}
-  IFB X <= Y THEN
-      {{                         }} ->>
-      {{                         }}
-    Z ::= Y - X
-      {{                         }}
-  ELSE
-      {{                         }} ->>
-      {{                         }}
-    Y ::= X + Z
-      {{                         }}
-  FI
-    {{ Y = X + Z }}
-*)
-
-
-(* ####################################################### *)
-(** ** Example: Reduce to Zero (Trivial Loop) *)
-
-(** Here is a [WHILE] loop that is so simple it needs no
-    invariant (i.e., the invariant [True] will do the job).
- (1)      {{ True }}
-        WHILE X <> 0 DO
- (2)        {{ True /\ X <> 0 }} ->>
- (3)        {{ True }}
-          X ::= X - 1
- (4)        {{ True }}
-        END
- (5)      {{ True /\ X = 0 }} ->>
- (6)      {{ X = 0 }}
-The decorations can be constructed as follows:
-  - Start with the outer precondition (1) and postcondition (6).
-  - Following the format dictated by the [hoare_while] rule, we copy
-    (1) to (4). We conjoin (1) with the guard to obtain (2) and with
-    the negation of the guard to obtain (5). Note that, because the
-    outer postcondition (6) does not syntactically match (5), we need a
-    trivial use of the consequence rule from (5) to (6).
-  - Assertion (3) is the same as (4), because [X] does not appear in
-    [4], so the substitution in the assignment rule is trivial.
-  - Finally, the implication between (2) and (3) is also trivial.
-*)
-
-(** From this informal proof, it is easy to read off a _formal_ proof
-    in terms of the Hoare rules: *)
-
-Definition reduce_to_zero' : com :=
-  WHILE BNot (BEq (AId X) (ANum 0)) DO
-    X ::= AMinus (AId X) (ANum 1)
-  END.
-
-Theorem reduce_to_zero_correct' : 
-  {{fun st => True}}
-  reduce_to_zero'
-  {{fun st => st X = 0}}.
-Proof.
-  (* Note that we do NOT unfold the definition of hoare_triple
-     anywhere in this proof! The goal is to use only the Hoare
-     rules. *)
-  unfold reduce_to_zero'.
-  (* First we need to transform the postcondition so
-     that hoare_while will apply. *)
-  eapply hoare_consequence_post.
-  apply hoare_while.
-  Case "Loop body preserves invariant".
-    (* Need to massage precondition before [hoare_asgn] applies *)
-    eapply hoare_consequence_pre. apply hoare_asgn.
-    (* Proving trivial implication (2) ->> (3) *)
-    intros st [HT Hbp]. unfold assn_sub. apply I.
-  Case "Invariant and negated guard imply postcondition".
-    intros st [Inv GuardFalse].
-    unfold bassn in GuardFalse. simpl in GuardFalse.
-    (* SearchAbout helps to find the right lemmas *)
-    SearchAbout [not true]. 
-    rewrite not_true_iff_false in GuardFalse. 
-    SearchAbout [negb false]. 
-    rewrite negb_false_iff in GuardFalse.
-    SearchAbout [beq_nat true]. 
-    apply beq_nat_true in GuardFalse.
-    apply GuardFalse. Qed.
-
-(* ####################################################### *)
-(** ** Example: Division *)
-
-
-(** The following Imp program calculates the integer division and
-    remainder of two numbers [a] and [b] that are arbitrary constants
-    in the program.
-  X ::= a;
-  Y ::= 0;
-  WHILE b <= X DO
-    X ::= X - b;
-    Y ::= Y + 1
-  END;
-    In other words, if we replace [a] and [b] by concrete numbers and
-    execute the program, it will terminate with the variable [X] set
-    to the remainder when [a] is divided by [b] and [Y] set to the
-    quotient.
-
-    In order to give a specification to this program we need to
-    remember that dividing [a] by [b] produces a reminder [X] and a
-    quotient [Y] so that [b * Y + X = a /\ X > b]. It turns out that
-    we get lucky with this program and don't have to think very hard
-    about the loop invariant: the invariant is the just first conjunct
-    [b * Y + X = a], so we use that to decorate the program.
-
- (1)    {{ True }} ->>
- (2)    {{ b * 0 + a = a }}
-      X ::= a;
- (3)    {{ b * 0 + X = a }}
-      Y ::= 0;
- (4)    {{ b * Y + X = a }}
-      WHILE b <= X DO
- (5)      {{ b * Y + X = a /\ b <= X }} ->>
- (6)      {{ b * (Y + 1) + (X - b) = a }} 
-        X ::= X - b;
- (7)      {{ b * (Y + 1) + X = a }}
-        Y ::= Y + 1
- (8)      {{ b * Y + X = a }}
-      END
- (9)    {{ b * Y + X = a /\ X < b }}
-
-    Assertions (4), (5), (8), and (9) are derived mechanically from
-    the invariant and the loop's guard. Assertions (8), (7), and (6)
-    are derived using the assignment rule going backwards from (8) to
-    (6). Assertions (4), (3), and (2) are again backwards applications
-    of the assignment rule.
-
-    Now that we've decorated the program it only remains to check that
-    the two uses of the consequence rule are correct -- i.e., that (1)
-    implies (2) and that (5) implies (6).  This is indeed the case, so
-    we have a valid decorated program.
-*)
-
-(* ####################################################### *)
-(** * Finding Loop Invariants *)
-
-(** Once the outermost precondition and postcondition are chosen, the
-    only creative part in verifying programs with Hoare Logic is
-    finding the right loop invariants.  The reason this is difficult
-    is the same as the reason that doing inductive mathematical proofs
-    requires creativity: strengthening the loop invariant (or the
-    induction hypothesis) means that you have a stronger assumption to
-    work with when trying to establish the postcondition of the loop
-    body (complete the induction step of the proof), but it also means
-    that the loop body postcondition itself is harder to prove!
-
-    This section is dedicated to teaching you how to approach the
-    challenge of finding loop invariants using a series of examples
-    and exercises. *)
-
-(** ** Example: Slow Subtraction *)
-
-(** The following program subtracts the value of [X] from the value of
-    [Y] by repeatedly decrementing both [X] and [Y]. We want to verify its
-    correctness with respect to the following specification:
-             {{ X = x /\ Y = y }}
-           WHILE X <> 0 DO
-             Y ::= Y - 1;
-             X ::= X - 1
-           END
-             {{ Y = y - x }}
-
-    To verify this program we need to find an invariant [I] for the
-    loop. As a first step we can leave [I] as an unknown and build a
-    _skeleton_ for the proof by applying backward the rules for local
-    consistency. This process leads to the following skeleton:
-    (1)      {{ X = x /\ Y = y }}  ->>     (a)
-    (2)      {{ I }}
-           WHILE X <> 0 DO
-    (3)        {{ I /\ X <> 0 }}  ->>      (c)
-    (4)        {{ I[X |-> X-1][Y |-> Y-1] }}
-             Y ::= Y - 1;
-    (5)        {{ I[X |-> X-1] }}
-             X ::= X - 1
-    (6)        {{ I }}
-           END
-    (7)      {{ I /\ X = 0 }}  ->>         (b)
-    (8)      {{ Y = y - x }}
-
-    By examining this skeleton, we can see that any valid [I] will
-    have to respect three conditions:
-    - (a) it must be weak enough to be implied by the loop's
-      precondition, i.e. (1) must imply (2);
-    - (b) it must be strong enough to imply the loop's postcondition,
-      i.e. (7) must imply (8);
-    - (c) it must be preserved by one iteration of the loop, i.e. (3)
-      must imply (4). *)
-
-
-(** These conditions are actually independent of the particular
-    program and specification we are considering. Indeed, every loop
-    invariant has to satisfy them. One way to find an invariant that
-    simultaneously satisfies these three conditions is by using an
-    iterative process: start with a "candidate" invariant (e.g. a
-    guess or a heuristic choice) and check the three conditions above;
-    if any of the checks fails, try to use the information that we get
-    from the failure to produce another (hopefully better) candidate
-    invariant, and repeat the process.
-
-    For instance, in the reduce-to-zero example above, we saw that,
-    for a very simple loop, choosing [True] as an invariant did the
-    job. So let's try it again here!  I.e., let's instantiate [I] with
-    [True] in the skeleton above see what we get...
-    (1)      {{ X = x /\ Y = y }} ->>       (a - OK)
-    (2)      {{ True }}
-           WHILE X <> 0 DO
-    (3)        {{ True /\ X <> 0 }}  ->>    (c - OK)
-    (4)        {{ True }}
-             Y ::= Y - 1;
-    (5)        {{ True }}
-             X ::= X - 1
-    (6)        {{ True }}
-           END
-    (7)      {{ True /\ X = 0 }}  ->>       (b - WRONG!)
-    (8)      {{ Y = y - x }}
-
-    While conditions (a) and (c) are trivially satisfied,
-    condition (b) is wrong, i.e. it is not the case that (7) [True /\
-    X = 0] implies (8) [Y = y - x].  In fact, the two assertions are
-    completely unrelated and it is easy to find a counterexample (say,
-    [Y = X = x = 0] and [y = 1]).
-
-    If we want (b) to hold, we need to strengthen the invariant so
-    that it implies the postcondition (8).  One very simple way to do
-    this is to let the invariant _be_ the postcondition.  So let's
-    return to our skeleton, instantiate [I] with [Y = y - x], and
-    check conditions (a) to (c) again.
-    (1)      {{ X = x /\ Y = y }}  ->>          (a - WRONG!)
-    (2)      {{ Y = y - x }}
-           WHILE X <> 0 DO
-    (3)        {{ Y = y - x /\ X <> 0 }}  ->>   (c - WRONG!)
-    (4)        {{ Y - 1 = y - x }}
-             Y ::= Y - 1;
-    (5)        {{ Y = y - x }}
-             X ::= X - 1
-    (6)        {{ Y = y - x }}
-           END
-    (7)      {{ Y = y - x /\ X = 0 }}  ->>      (b - OK)
-    (8)      {{ Y = y - x }}
-
-    This time, condition (b) holds trivially, but (a) and (c) are
-    broken. Condition (a) requires that (1) [X = x /\ Y = y]
-    implies (2) [Y = y - x].  If we substitute [X] by [x] we have to
-    show that [x = y - x] for arbitrary [x] and [y], which does not
-    hold (for instance, when [x = y = 1]).  Condition (c) requires that
-    [y - x - 1 = y - x], which fails, for instance, for [y = 1] and [x =
-    0]. So, although [Y = y - x] holds at the end of the loop, it does
-    not hold from the start, and it doesn't hold on each iteration;
-    it is not a correct invariant.
-
-    This failure is not very surprising: the variable [Y] changes
-    during the loop, while [x] and [y] are constant, so the assertion
-    we chose didn't have much chance of being an invariant!  To do
-    better, we need to generalize (8) to some statement that is
-    equivalent to (8) when [X] is [0], since this will be the case
-    when the loop terminates, and that "fills the gap" in some
-    appropriate way when [X] is nonzero.  Looking at how the loop
-    works, we can observe that [X] and [Y] are decremented together
-    until [X] reaches [0].  So, if [X = 2] and [Y = 5] initially,
-    after one iteration of the loop we obtain [X = 1] and [Y = 4];
-    after two iterations [X = 0] and [Y = 3]; and then the loop stops.
-    Notice that the difference between [Y] and [X] stays constant
-    between iterations; initially, [Y = y] and [X = x], so this
-    difference is always [y - x].  So let's try instantiating [I] in
-    the skeleton above with [Y - X = y - x].
-    (1)      {{ X = x /\ Y = y }}  ->>               (a - OK)
-    (2)      {{ Y - X = y - x }}
-           WHILE X <> 0 DO
-    (3)        {{ Y - X = y - x /\ X <> 0 }}  ->>    (c - OK)
-    (4)        {{ (Y - 1) - (X - 1) = y - x }}
-             Y ::= Y - 1;
-    (5)        {{ Y - (X - 1) = y - x }}
-             X ::= X - 1
-    (6)        {{ Y - X = y - x }}
-           END
-    (7)      {{ Y - X = y - x /\ X = 0 }}  ->>       (b - OK)
-    (8)      {{ Y = y - x }}
-
-    Success!  Conditions (a), (b) and (c) all hold now.  (To
-    verify (c), we need to check that, under the assumption that [X <>
-    0], we have [Y - X = (Y - 1) - (X - 1)]; this holds for all
-    natural numbers [X] and [Y].) *)
-
-(* ####################################################### *)
-(** ** Exercise: Slow Assignment *)
-
-(** **** Exercise: 2 stars (slow_assignment) *)
-(** A roundabout way of assigning a number currently stored in [X] to
-    the variable [Y] is to start [Y] at [0], then decrement [X] until
-    it hits [0], incrementing [Y] at each step. Here is a program that
-    implements this idea:
-      {{ X = x }}
-    Y ::= 0;
-    WHILE X <> 0 DO
-      X ::= X - 1;
-      Y ::= Y + 1;
-    END
-      {{ Y = x }}
-    Write an informal decorated program showing that this is correct. *)
-
-(* FILL IN HERE *)
-(** [] *)
-
-(* ####################################################### *)
-(** ** Exercise: Slow Addition *)
-
-
-(** **** Exercise: 3 stars, optional (add_slowly_decoration) *)
-(** The following program adds the variable X into the variable Z
-    by repeatedly decrementing X and incrementing Z.
-  WHILE X <> 0 DO
-     Z ::= Z + 1;
-     X ::= X - 1
-  END
-
-    Following the pattern of the [subtract_slowly] example above, pick
-    a precondition and postcondition that give an appropriate
-    specification of [add_slowly]; then (informally) decorate the
-    program accordingly. *)
-
-(* FILL IN HERE *)
-(** [] *)
-
-(* ####################################################### *)
-(** ** Example: Parity *)
-
-
-(** Here is a cute little program for computing the parity of the
-    value initially stored in [X] (due to Daniel Cristofani).
-    {{ X = x }}
-  WHILE 2 <= X DO
-    X ::= X - 2
-  END
-    {{ X = parity x }}
-    The mathematical [parity] function used in the specification is
-    defined in Coq as follows: *)
-
-Fixpoint parity x :=
-  match x with
-  | 0 => 0
-  | 1 => 1
-  | S (S x') => parity x'
-  end.
-
-(** The postcondition does not hold at the beginning of the loop,
-    since [x = parity x] does not hold for an arbitrary [x], so we
-    cannot use that as an invariant.  To find an invariant that works,
-    let's think a bit about what this loop does.  On each iteration it
-    decrements [X] by [2], which preserves the parity of [X].  So the
-    parity of [X] does not change, i.e. it is invariant.  The initial
-    value of [X] is [x], so the parity of [X] is always equal to the
-    parity of [x]. Using [parity X = parity x] as an invariant we
-    obtain the following decorated program:
-    {{ X = x }} ->>                              (a - OK)
-    {{ parity X = parity x }}
-  WHILE 2 <= X DO
-      {{ parity X = parity x /\ 2 <= X }}  ->>    (c - OK)
-      {{ parity (X-2) = parity x }}
-    X ::= X - 2
-      {{ parity X = parity x }}
-  END
-    {{ parity X = parity x /\ X < 2 }}  ->>       (b - OK)
-    {{ X = parity x }}
-
-    With this invariant, conditions (a), (b), and (c) are all
-    satisfied. For verifying (b), we observe that, when [X < 2], we
-    have [parity X = X] (we can easily see this in the definition of
-    [parity]).  For verifying (c), we observe that, when [2 <= X], we
-    have [parity X = parity (X-2)]. *)
-
-
-(** **** Exercise: 3 stars, optional (parity_formal) *)
-(** Translate this proof to Coq. Refer to the reduce-to-zero example
-    for ideas. You might find the following two lemmas useful: *)
-
-Lemma parity_ge_2 : forall x,
-  2 <= x ->
-  parity (x - 2) = parity x.
-Proof.
-  induction x; intro. reflexivity.
-  destruct x. inversion H. inversion H1.
-  simpl. rewrite <- minus_n_O. reflexivity.
-Qed.
-
-Lemma parity_lt_2 : forall x,
-  ~ 2 <= x ->
-  parity (x) = x.
-Proof.
-  intros. induction x. reflexivity. destruct x. reflexivity.
-    apply ex_falso_quodlibet. apply H. omega.
-Qed.
-
-Theorem parity_correct : forall x,
-    {{ fun st => st X = x }}
-  WHILE BLe (ANum 2) (AId X) DO
-    X ::= AMinus (AId X) (ANum 2)
-  END
-    {{ fun st => st X = parity x }}.
-Proof.
-  (* FILL IN HERE *) Admitted.
-(** [] *)
-
-(* ####################################################### *) 
-(** ** Example: Finding Square Roots *)
-
-
-(** The following program computes the square root of [X]
-    by naive iteration:
-      {{ X=x }}
-    Z ::= 0;
-    WHILE (Z+1)*(Z+1) <= X DO
-      Z ::= Z+1
-    END
-      {{ Z*Z<=x /\ x<(Z+1)*(Z+1) }}
-
-    As above, we can try to use the postcondition as a candidate
-    invariant, obtaining the following decorated program:
- (1)  {{ X=x }}  ->>           (a - second conjunct of (2) WRONG!)
- (2)  {{ 0*0 <= x /\ x<1*1 }} 
-    Z ::= 0;
- (3)  {{ Z*Z <= x /\ x<(Z+1)*(Z+1) }}
-    WHILE (Z+1)*(Z+1) <= X DO
- (4)    {{ Z*Z<=x /\ (Z+1)*(Z+1)<=X }}  ->>           (c - WRONG!)
- (5)    {{ (Z+1)*(Z+1)<=x /\ x<(Z+2)*(Z+2) }} 
-      Z ::= Z+1
- (6)    {{ Z*Z<=x /\ x<(Z+1)*(Z+1) }}
-    END
- (7)  {{ Z*Z<=x /\ x<(Z+1)*(Z+1) /\ X<(Z+1)*(Z+1) }}  ->> (b - OK)
- (8)  {{ Z*Z<=x /\ x<(Z+1)*(Z+1) }}
-
-    This didn't work very well: both conditions (a) and (c) failed.
-    Looking at condition (c), we see that the second conjunct of (4)
-    is almost the same as the first conjunct of (5), except that (4)
-    mentions [X] while (5) mentions [x]. But note that [X] is never
-    assigned in this program, so we should have [X=x], but we didn't
-    propagate this information from (1) into the loop invariant.
-    Looking at the second conjunct of (8), it seems quite hopeless as
-    an invariant -- and we don't even need it, since we can obtain it
-    from the negation of the guard (third conjunct in (7)), again
-    under the assumption that [X=x].  So we now try [X=x /\ Z*Z <= x]
-    as the loop invariant:
-      {{ X=x }}  ->>                                      (a - OK)
-      {{ X=x /\ 0*0 <= x }}
-    Z ::= 0;
-      {{ X=x /\ Z*Z <= x }}
-    WHILE (Z+1)*(Z+1) <= X DO
-        {{ X=x /\ Z*Z<=x /\ (Z+1)*(Z+1)<=X }}  ->>        (c - OK)
-        {{ X=x /\ (Z+1)*(Z+1)<=x }} 
-      Z ::= Z+1
-        {{ X=x /\ Z*Z<=x }} 
-    END
-      {{ X=x /\ Z*Z<=x /\ X<(Z+1)*(Z+1) }}  ->>           (b - OK)
-      {{ Z*Z<=x /\ x<(Z+1)*(Z+1) }}
-
-    This works, since conditions (a), (b), and (c) are now all
-    trivially satisfied. 
-
-    Very often, if a variable is used in a loop in a read-only
-    fashion (i.e., it is referred to by the program or by the
-    specification and it is not changed by the loop) it is necessary
-    to add the fact that it doesn't change to the loop invariant. *)
-
-(* ####################################################### *)
-(** ** Example: Squaring *)
-
-
-(** Here is a program that squares [X] by repeated addition:
-
-  {{ X = x }}
-  Y ::= 0;
-  Z ::= 0;
-  WHILE  Y  <>  X  DO
-    Z ::= Z + X;
-    Y ::= Y + 1
-  END
-  {{ Z = x*x }}
-    The first thing to note is that the loop reads [X] but doesn't
-    change its value. As we saw in the previous example, in such cases
-    it is a good idea to add [X = x] to the invariant. The other thing
-    we often use in the invariant is the postcondition, so let's add
-    that too, leading to the invariant candidate [Z = x * x /\ X = x].
-      {{ X = x }} ->>                            (a - WRONG)
-      {{ 0 = x*x /\ X = x }}
-    Y ::= 0;
-      {{ 0 = x*x /\ X = x }}
-    Z ::= 0;
-      {{ Z = x*x /\ X = x }}
-    WHILE Y <> X DO
-        {{ Z = Y*x /\ X = x /\ Y <> X }} ->>     (c - WRONG)
-        {{ Z+X = x*x /\ X = x }}
-      Z ::= Z + X;
-        {{ Z = x*x /\ X = x }}
-      Y ::= Y + 1
-        {{ Z = x*x /\ X = x }}
-    END
-      {{ Z = x*x /\ X = x /\ Y = X }} ->>         (b - OK)
-      {{ Z = x*x }}
-
-    Conditions (a) and (c) fail because of the [Z = x*x] part.  While
-    [Z] starts at [0] and works itself up to [x*x], we can't expect
-    [Z] to be [x*x] from the start.  If we look at how [Z] progesses
-    in the loop, after the 1st iteration [Z = x], after the 2nd
-    iteration [Z = 2*x], and at the end [Z = x*x].  Since the variable
-    [Y] tracks how many times we go through the loop, we derive the
-    new invariant candidate [Z = Y*x /\ X = x].
-      {{ X = x }} ->>                               (a - OK)
-      {{ 0 = 0*x /\ X = x }}
-    Y ::= 0;
-      {{ 0 = Y*x /\ X = x }}
-    Z ::= 0;
-      {{ Z = Y*x /\ X = x }}
-    WHILE Y <> X DO
-        {{ Z = Y*x /\ X = x /\ Y <> X }} ->>        (c - OK)
-        {{ Z+X = (Y+1)*x /\ X = x }}
-      Z ::= Z + X;
-        {{ Z = (Y+1)*x /\ X = x }}
-      Y ::= Y + 1
-        {{ Z = Y*x /\ X = x }}
-    END
-      {{ Z = Y*x /\ X = x /\ Y = X }} ->>           (b - OK)
-      {{ Z = x*x }}
-
-    This new invariant makes the proof go through: all three
-    conditions are easy to check.
-
-    It is worth comparing the postcondition [Z = x*x] and the [Z =
-    Y*x] conjunct of the invariant. It is often the case that one has
-    to replace auxiliary variabes (parameters) with variables -- or
-    with expressions involving both variables and parameters (like
-    [x - Y]) -- when going from postconditions to invariants. *)
-
-(* ####################################################### *)
-(** ** Exercise: Factorial *)
-
-(** **** Exercise: 3 stars (factorial) *)
-(** Recall that [n!] denotes the factorial of [n] (i.e. [n! =
-    1*2*...*n]).  Here is an Imp program that calculates the factorial
-    of the number initially stored in the variable [X] and puts it in
-    the variable [Y]:
-    {{ X = x }} ;
-  Y ::= 1
-  WHILE X <> 0
-  DO
-     Y ::= Y * X
-     X ::= X - 1
-  END
-    {{ Y = x! }}
-
-    Fill in the blanks in following decorated program:
-    {{ X = x }} ->>
-    {{                                      }}
-  Y ::= 1;
-    {{                                      }}
-  WHILE X <> 0
-  DO   {{                                      }} ->>
-       {{                                      }}
-     Y ::= Y * X;
-       {{                                      }}
-     X ::= X - 1
-       {{                                      }} 
-  END
-    {{                                      }} ->>
-    {{ Y = x! }}
-*)
-
-
-(* ####################################################### *)
-(** ** Exercise: Two Loops *)
-
-
-(** **** Exercise: 3 stars (two_loops) *)
-(** Here is a very inefficient way of adding 3 numbers:
-  X ::= 0;
-  Y ::= 0;
-  Z ::= c;
-  WHILE X <> a DO
-    X ::= X + 1;
-    Z ::= Z + 1
-  END;
-  WHILE Y <> b DO
-    Y ::= Y + 1;
-    Z ::= Z + 1
-  END
-
-    Show that it does what it should by filling in the blanks in the
-    following decorated program.
-
-    {{ True }} ->>
-    {{                                        }}
-  X ::= 0;
-    {{                                        }}
-  Y ::= 0;
-    {{                                        }}
-  Z ::= c;
-    {{                                        }}
-  WHILE X <> a DO
-      {{                                        }} ->>
-      {{                                        }}
-    X ::= X + 1;
-      {{                                        }}
-    Z ::= Z + 1
-      {{                                        }}
-  END;
-    {{                                        }} ->>
-    {{                                        }}
-  WHILE Y <> b DO
-      {{                                        }} ->>
-      {{                                        }}
-    Y ::= Y + 1;
-      {{                                        }}
-    Z ::= Z + 1
-      {{                                        }}
-  END
-    {{                                        }} ->>
-    {{ Z = a + b + c }}
-*)
-
-
-(* ####################################################### *)
-(** ** Exercise: Power Series *)
-
-
-(** **** Exercise: 4 stars, optional (dpow2_down) *)
-(** Here is a program that computes the series:
-    [1 + 2 + 2^2 + ... + 2^x = 2^(x+1) - 1]
-  X ::= 0;
-  Y ::= 1;
-  Z ::= 1;
-  WHILE X <> x DO
-    Z ::= 2 * Z;
-    Y ::= Y + Z;
-    X ::= X + 1;
-  END
-    Write a decorated program for this. *)
-
-(* FILL IN HERE *)
-
-
-(* ####################################################### *) 
-(** * Weakest Preconditions (Advanced) *)
-
-(** Some Hoare triples are more interesting than others.
-    For example,
-      {{ False }}  X ::= Y + 1  {{ X <= 5 }}
-    is _not_ very interesting: although it is perfectly valid, it
-    tells us nothing useful.  Since the precondition isn't satisfied
-    by any state, it doesn't describe any situations where we can use
-    the command [X ::= Y + 1] to achieve the postcondition [X <= 5].
-
-    By contrast, 
-      {{ Y <= 4 /\ Z = 0 }}  X ::= Y + 1 {{ X <= 5 }}
-    is useful: it tells us that, if we can somehow create a situation
-    in which we know that [Y <= 4 /\ Z = 0], then running this command
-    will produce a state satisfying the postcondition.  However, this
-    triple is still not as useful as it could be, because the [Z = 0]
-    clause in the precondition actually has nothing to do with the
-    postcondition [X <= 5].  The _most_ useful triple (for a given
-    command and postcondition) is this one:
-      {{ Y <= 4 }}  X ::= Y + 1  {{ X <= 5 }}
-    In other words, [Y <= 4] is the _weakest_ valid precondition of
-    the command [X ::= Y + 1] for the postcondition [X <= 5]. *)
- 
-(** In general, we say that "[P] is the weakest precondition of
-    command [c] for postcondition [Q]" if [{{P}} c {{Q}}] and if,
-    whenever [P'] is an assertion such that [{{P'}} c {{Q}}], we have
-    [P' st] implies [P st] for all states [st].  *)
-
-Definition is_wp P c Q :=
-  {{P}} c {{Q}} /\
-  forall P', {{P'}} c {{Q}} -> (P' ->> P).
-
-(** That is, [P] is the weakest precondition of [c] for [Q]
-    if (a) [P] _is_ a precondition for [Q] and [c], and (b) [P] is the
-    _weakest_ (easiest to satisfy) assertion that guarantees [Q] after
-    executing [c]. *)
-
-(** **** Exercise: 1 star, advanced (wp) *)
-(** What are the weakest preconditions of the following commands
-   for the following postconditions?
-  1) {{ ? }}  SKIP  {{ X = 5 }}
-
-  2) {{ ? }}  X ::= Y + Z {{ X = 5 }}
-
-  3) {{ ? }}  X ::= Y  {{ X = Y }}
-
-  4) {{ ? }}  
-     IFB X == 0 THEN Y ::= Z + 1 ELSE Y ::= W + 2 FI
-     {{ Y = 5 }}
-
-  5) {{ ? }}  
-     X ::= 5
-     {{ X = 0 }}
-
-  6) {{ ? }}  
-     WHILE True DO X ::= 0 END
-     {{ X = 0 }}
-*)
-(* FILL IN HERE *)
-(** [] *)
-
-(** **** Exercise: 3 stars, advanced, optional (is_wp_formal) *)
-(** Prove formally using the definition of [hoare_triple] that [Y <= 4]
-   is indeed the weakest precondition of [X ::= Y + 1] with respect to
-   postcondition [X <= 5]. *)
-
-Theorem is_wp_example :
-  is_wp (fun st => st Y <= 4)
-    (X ::= APlus (AId Y) (ANum 1)) (fun st => st X <= 5).
-Proof.
-  (* FILL IN HERE *) Admitted.
-(** [] *)
-
-(** **** Exercise: 2 stars, advanced (hoare_asgn_weakest) *)
-(** Show that the precondition in the rule [hoare_asgn] is in fact the
-    weakest precondition. *)
-
-Theorem hoare_asgn_weakest : forall Q X a,
-  is_wp (Q [X |-> a]) (X ::= a) Q.
-Proof.
-(* FILL IN HERE *) Admitted.
-(** [] *)
-
-(** **** Exercise: 2 stars, advanced (hoare_havoc_weakest) *)
-(** Show that your [havoc_pre] rule from the [himp_hoare] exercise
-    above returns the weakest precondition. *)
-Module Himp2.
-Import Himp.
-
-Lemma hoare_havoc_weakest : forall (P Q : Assertion) (X : id),
-  {{ P }} HAVOC X {{ Q }} ->
-  P ->> havoc_pre X Q.
-Proof.
-(* FILL IN HERE *) Admitted.
-End Himp2.
-(** [] *)
-
-(* ####################################################### *)
-(** * Formal Decorated Programs (Advanced) *)
-
-(** The informal conventions for decorated programs amount to a way of
-    displaying Hoare triples in which commands are annotated with
-    enough embedded assertions that checking the validity of the
-    triple is reduced to simple logical and algebraic calculations
-    showing that some assertions imply others.  In this section, we
-    show that this informal presentation style can actually be made
-    completely formal and indeed that checking the validity of
-    decorated programs can mostly be automated.  *)
-
-(** ** Syntax *)
-
-(** The first thing we need to do is to formalize a variant of the
-    syntax of commands with embedded assertions.  We call the new
-    commands _decorated commands_, or [dcom]s. *)
-
-Inductive dcom : Type :=
-  | DCSkip :  Assertion -> dcom
-  | DCSeq : dcom -> dcom -> dcom
-  | DCAsgn : id -> aexp ->  Assertion -> dcom
-  | DCIf : bexp ->  Assertion -> dcom ->  Assertion -> dcom
-           -> Assertion-> dcom
-  | DCWhile : bexp -> Assertion -> dcom -> Assertion -> dcom
-  | DCPre : Assertion -> dcom -> dcom
-  | DCPost : dcom -> Assertion -> dcom.
-
-Tactic Notation "dcom_cases" tactic(first) ident(c) :=
-  first;
-  [ Case_aux c "Skip" | Case_aux c "Seq" | Case_aux c "Asgn"
-  | Case_aux c "If" | Case_aux c "While"
-  | Case_aux c "Pre" | Case_aux c "Post" ].
-
-Notation "'SKIP' {{ P }}" 
-      := (DCSkip P) 
-      (at level 10) : dcom_scope.
-Notation "l '::=' a {{ P }}" 
-      := (DCAsgn l a P) 
-      (at level 60, a at next level) : dcom_scope.
-Notation "'WHILE' b 'DO' {{ Pbody }} d 'END' {{ Ppost }}" 
-      := (DCWhile b Pbody d Ppost) 
-      (at level 80, right associativity) : dcom_scope.
-Notation "'IFB' b 'THEN' {{ P }} d 'ELSE' {{ P' }} d' 'FI' {{ Q }}" 
-      := (DCIf b P d P' d' Q) 
-      (at level 80, right associativity)  : dcom_scope.
-Notation "'->>' {{ P }} d"
-      := (DCPre P d) 
-      (at level 90, right associativity)  : dcom_scope.
-Notation "{{ P }} d" 
-      := (DCPre P d) 
-      (at level 90)  : dcom_scope.
-Notation "d '->>' {{ P }}"
-      := (DCPost d P) 
-      (at level 80, right associativity)  : dcom_scope.
-Notation " d ; d' " 
-      := (DCSeq d d') 
-      (at level 80, right associativity)  : dcom_scope.
-
-Delimit Scope dcom_scope with dcom.
-
-(** To avoid clashing with the existing [Notation] definitions
-    for ordinary [com]mands, we introduce these notations in a special
-    scope called [dcom_scope], and we wrap examples with the
-    declaration [% dcom] to signal that we want the notations to be
-    interpreted in this scope.  
-
-    Careful readers will note that we've defined two notations for the
-    [DCPre] constructor, one with and one without a [->>].  The
-    "without" version is intended to be used to supply the initial
-    precondition at the very top of the program. *)
-
-Example dec_while : dcom := (
-  {{ fun st => True }}
-  WHILE (BNot (BEq (AId X) (ANum 0))) 
-  DO
-    {{ fun st => True /\ st X <> 0}}
-    X ::= (AMinus (AId X) (ANum 1)) 
-    {{ fun _ => True }}
-  END
-  {{ fun st => True /\ st X = 0}} ->>
-  {{ fun st => st X = 0 }}
-) % dcom.
-
-(** It is easy to go from a [dcom] to a [com] by erasing all
-    annotations. *)
-
-Fixpoint extract (d:dcom) : com :=
-  match d with
-  | DCSkip _           => SKIP
-  | DCSeq d1 d2        => (extract d1 ; extract d2) 
-  | DCAsgn X a _       => X ::= a
-  | DCIf b _ d1 _ d2 _ => IFB b THEN extract d1 ELSE extract d2 FI
-  | DCWhile b _ d _    => WHILE b DO extract d END
-  | DCPre _ d          => extract d
-  | DCPost d _         => extract d
-  end.
-
-(** The choice of exactly where to put assertions in the definition of
-    [dcom] is a bit subtle.  The simplest thing to do would be to
-    annotate every [dcom] with a precondition and postcondition.  But
-    this would result in very verbose programs with a lot of repeated
-    annotations: for example, a program like [SKIP;SKIP] would have to
-    be annotated as
-        {{P}} ({{P}} SKIP {{P}}) ; ({{P}} SKIP {{P}}) {{P}},
-    with pre- and post-conditions on each [SKIP], plus identical pre-
-    and post-conditions on the semicolon!  
-
-    Instead, the rule we've followed is this:
-
-       - The _post_-condition expected by each [dcom] [d] is embedded in [d]
-
-       - The _pre_-condition is supplied by the context. *)
-
-(** In other words, the invariant of the representation is that a
-    [dcom] [d] together with a precondition [P] determines a Hoare
-    triple [{{P}} (extract d) {{post d}}], where [post] is defined as
-    follows: *)
-
-Fixpoint post (d:dcom) : Assertion :=
-  match d with
-  | DCSkip P                => P
-  | DCSeq d1 d2             => post d2
-  | DCAsgn X a Q            => Q
-  | DCIf  _ _ d1 _ d2 Q     => Q
-  | DCWhile b Pbody c Ppost => Ppost
-  | DCPre _ d               => post d
-  | DCPost c Q              => Q
-  end.
-
-(** We can define a similar function that extracts the "initial
-    precondition" from a decorated program. *)
-
-Fixpoint pre (d:dcom) : Assertion :=
-  match d with
-  | DCSkip P                => fun st => True
-  | DCSeq c1 c2             => pre c1
-  | DCAsgn X a Q            => fun st => True
-  | DCIf  _ _ t _ e _       => fun st => True
-  | DCWhile b Pbody c Ppost => fun st => True
-  | DCPre P c               => P
-  | DCPost c Q              => pre c
-  end.
-
-(** This function is not doing anything sophisticated like calculating
-    a weakest precondition; it just recursively searches for an
-    explicit annotation at the very beginning of the program,
-    returning default answers for programs that lack an explicit
-    precondition (like a bare assignment or [SKIP]).  
-
-    Using [pre] and [post], and assuming that we adopt the convention
-    of always supplying an explicit precondition annotation at the
-    very beginning of our decorated programs, we can express what it
-    means for a decorated program to be correct as follows: *)
-
-Definition dec_correct (d:dcom) := 
-  {{pre d}} (extract d) {{post d}}.
-
-(** To check whether this Hoare triple is _valid_, we need a way to
-    extract the "proof obligations" from a decorated program.  These
-    obligations are often called _verification conditions_, because
-    they are the facts that must be verified to see that the
-    decorations are logically consistent and thus add up to a complete
-    proof of correctness. *)
-
-(** ** Extracting Verification Conditions *)
-
-(** The function [verification_conditions] takes a [dcom] [d] together
-    with a precondition [P] and returns a _proposition_ that, if it
-    can be proved, implies that the triple [{{P}} (extract d) {{post d}}]
-    is valid.  It does this by walking over [d] and generating a big
-    conjunction including all the "local checks" that we listed when
-    we described the informal rules for decorated programs.
-    (Strictly speaking, we need to massage the informal rules a little
-    bit to add some uses of the rule of consequence, but the
-    correspondence should be clear.) *)
-
-Fixpoint verification_conditions (P : Assertion) (d:dcom) : Prop :=
-  match d with
-  | DCSkip Q          => 
-      (P ->> Q)
-  | DCSeq d1 d2      => 
-      verification_conditions P d1
-      /\ verification_conditions (post d1) d2
-  | DCAsgn X a Q      =>
-      (P ->> Q [X |-> a])
-  | DCIf b P1 d1 P2 d2 Q =>
-      ((fun st => P st /\ bassn b st) ->> P1)
-      /\ ((fun st => P st /\ ~ (bassn b st)) ->> P2)
-      /\ (Q <<->> post d1) /\ (Q <<->> post d2)
-      /\ verification_conditions P1 d1
-      /\ verification_conditions P2 d2
-  | DCWhile b Pbody d Ppost      => 
-      (* post d is the loop invariant and the initial precondition *)
-      (P ->> post d)  
-      /\ (Pbody <<->> (fun st => post d st /\ bassn b st))
-      /\ (Ppost <<->> (fun st => post d st /\ ~(bassn b st)))
-      /\ verification_conditions Pbody d
-  | DCPre P' d         => 
-      (P ->> P') /\ verification_conditions P' d
-  | DCPost d Q        => 
-      verification_conditions P d /\ (post d ->> Q)
-  end.
-
-(** And now, the key theorem, which captures the claim that the
-    [verification_conditions] function does its job correctly.  Not
-    surprisingly, we need all of the Hoare Logic rules in the
-    proof. *)
-(** We have used _in_ variants of several tactics before to
-    apply them to values in the context rather than the goal. An
-    extension of this idea is the syntax [tactic in *], which applies
-    [tactic] in the goal and every hypothesis in the context.  We most
-    commonly use this facility in conjunction with the [simpl] tactic,
-    as below. *)
-
-Theorem verification_correct : forall d P, 
-  verification_conditions P d -> {{P}} (extract d) {{post d}}.
-Proof.
-  dcom_cases (induction d) Case; intros P H; simpl in *.
-  Case "Skip".
-    eapply hoare_consequence_pre.
-      apply hoare_skip.
-      assumption.
-  Case "Seq". 
-    inversion H as [H1 H2]. clear H. 
-    eapply hoare_seq. 
-      apply IHd2. apply H2.
-      apply IHd1. apply H1.
-  Case "Asgn". 
-    eapply hoare_consequence_pre.
-      apply hoare_asgn.
-      assumption.
-  Case "If".
-    inversion H as [HPre1 [HPre2 [[Hd11 Hd12] 
-                                  [[Hd21 Hd22] [HThen HElse]]]]].
-    clear H.
-    apply IHd1 in HThen. clear IHd1.
-    apply IHd2 in HElse. clear IHd2.
-    apply hoare_if.
-      eapply hoare_consequence_pre; eauto.
-      eapply hoare_consequence_post; eauto.
-      eapply hoare_consequence_pre; eauto.
-      eapply hoare_consequence_post; eauto.
-  Case "While".
-    inversion H as [Hpre [[Hbody1 Hbody2] [[Hpost1 Hpost2]  Hd]]];
-    subst; clear H.
-    eapply hoare_consequence_pre; eauto.
-    eapply hoare_consequence_post; eauto.
-    apply hoare_while.
-    eapply hoare_consequence_pre; eauto.
-  Case "Pre".
-    inversion H as [HP Hd]; clear H. 
-    eapply hoare_consequence_pre. apply IHd. apply Hd. assumption.
-  Case "Post".
-    inversion H as [Hd HQ]; clear H.
-    eapply hoare_consequence_post. apply IHd. apply Hd. assumption.
-Qed.
-
-(** ** Examples *)
-
-(** The propositions generated by [verification_conditions] are fairly
-    big, and they contain many conjuncts that are essentially trivial. *)
-
-Eval simpl in (verification_conditions (fun st => True) dec_while).
-(**
-==>
-(((fun _ : state => True) ->> (fun _ : state => True)) /\
- ((fun _ : state => True) ->> (fun _ : state => True)) /\
- (fun st : state => True /\ bassn (BNot (BEq (AId X) (ANum 0))) st) =
- (fun st : state => True /\ bassn (BNot (BEq (AId X) (ANum 0))) st) /\
- (fun st : state => True /\ ~ bassn (BNot (BEq (AId X) (ANum 0))) st) =
- (fun st : state => True /\ ~ bassn (BNot (BEq (AId X) (ANum 0))) st) /\
- (fun st : state => True /\ bassn (BNot (BEq (AId X) (ANum 0))) st) ->>
- (fun _ : state => True) [X |-> AMinus (AId X) (ANum 1)]) /\
-(fun st : state => True /\ ~ bassn (BNot (BEq (AId X) (ANum 0))) st) ->>
-(fun st : state => st X = 0) 
-*)
-
-(** In principle, we could certainly work with them using just the
-    tactics we have so far, but we can make things much smoother with
-    a bit of automation.  We first define a custom [verify] tactic
-    that applies splitting repeatedly to turn all the conjunctions
-    into separate subgoals and then uses [omega] and [eauto] (a handy
-    general-purpose automation tactic that we'll discuss in detail
-    later) to deal with as many of them as possible. *)
-
-Lemma ble_nat_true_iff : forall n m : nat,
-  ble_nat n m = true <-> n <= m.
-Proof.
-  intros n m. split. apply ble_nat_true.
-  generalize dependent m. induction n; intros m H. reflexivity.
-    simpl. destruct m. inversion H.
-    apply le_S_n in H. apply IHn. assumption.
-Qed.
-
-Lemma ble_nat_false_iff : forall n m : nat,
-  ble_nat n m = false <-> ~(n <= m).
-Proof.
-  intros n m. split. apply ble_nat_false.
-  generalize dependent m. induction n; intros m H.
-    apply ex_falso_quodlibet. apply H. apply le_0_n.
-    simpl. destruct m. reflexivity.
-    apply IHn. intro Hc. apply H. apply le_n_S. assumption.
-Qed.
-
-Tactic Notation "verify" :=
-  apply verification_correct; 
-  repeat split;
-  simpl; unfold assert_implies; 
-  unfold bassn in *; unfold beval in *; unfold aeval in *;
-  unfold assn_sub; intros;
-  repeat rewrite update_eq;
-  repeat (rewrite update_neq; [| reflexivity]);
-  simpl in *; 
-  repeat match goal with [H : _ /\ _ |- _] => destruct H end;
-  repeat rewrite not_true_iff_false in *;
-  repeat rewrite not_false_iff_true in *;
-  repeat rewrite negb_true_iff in *;
-  repeat rewrite negb_false_iff in *;
-  repeat rewrite beq_nat_true_iff in *;
-  repeat rewrite beq_nat_false_iff in *;
-  repeat rewrite ble_nat_true_iff in *;
-  repeat rewrite ble_nat_false_iff in *;
-  try subst;
-  repeat
-    match goal with
-      [st : state |- _] =>
-        match goal with
-          [H : st _ = _ |- _] => rewrite -> H in *; clear H
-        | [H : _ = st _ |- _] => rewrite <- H in *; clear H
-        end
-    end;
-  try eauto; try omega.
-
-(** What's left after [verify] does its thing is "just the interesting
-    parts" of checking that the decorations are correct. For very
-    simple examples [verify] immediately solves the goal (provided
-    that the annotations are correct). *)
-
-Theorem dec_while_correct :
-  dec_correct dec_while.
-Proof. verify. Qed.
-
-(** Another example (formalizing a decorated program we've seen
-    before): *)
-
-Example subtract_slowly_dec (x:nat) (z:nat) : dcom := (
-    {{ fun st => st X = x /\ st Z = z }} ->>
-    {{ fun st => st Z - st X = z - x }}
-  WHILE BNot (BEq (AId X) (ANum 0))
-  DO   {{ fun st => st Z - st X = z - x /\ st X <> 0 }} ->>
-       {{ fun st => (st Z - 1) - (st X - 1) = z - x }}
-     Z ::= AMinus (AId Z) (ANum 1)
-       {{ fun st => st Z - (st X - 1) = z - x }} ;
-     X ::= AMinus (AId X) (ANum 1) 
-       {{ fun st => st Z - st X = z - x }}
-  END
-    {{ fun st => st Z - st X = z - x /\ st X = 0 }} ->>
-    {{ fun st => st Z = z - x }}
-) % dcom.
-
-Theorem subtract_slowly_dec_correct : forall x z, 
-  dec_correct (subtract_slowly_dec x z).
-Proof. intros x z. verify. (* this grinds for a bit! *) Qed.
-
-(** **** Exercise: 3 stars, optional (slow_assignment_dec) *)
-
-(** A roundabout way of assigning a number currently stored in [X] to
-   the variable [Y] is to start [Y] at [0], then decrement [X] until it
-   hits [0], incrementing [Y] at each step.
-
-   Here is an informal decorated program that implements this idea
-   given a parameter [x]: 
-      {{ X = x }}
-    Y ::= 0;
-      {{ X = x /\ Y = 0 }} ->>
-      {{ Y + X = x }}
-    WHILE X <> 0 DO
-        {{ Y + X = x /\ X <> 0 }} ->>
-        {{ Y + (X - 1) + 1 = x }}
-      X ::= X - 1;
-        {{ Y + X + 1 = x }}
-      Y ::= Y + 1;
-        {{ Y + X = x }}
-    END
-      {{ Y + X = x /\ X = 0 }} ->>
-      {{ Y = x }}
-*)
-
-(** Write a corresponding formal decorated program (parametrized by [x])
-    and prove it correct. *)
-
-Example slow_assignment_dec (x:nat) : dcom :=
-(* FILL IN HERE *) admit.
-
-Theorem slow_assignment_dec_correct : forall x,
-  dec_correct (slow_assignment_dec x).
-Proof. (* FILL IN HERE *) Admitted.
-(** [] *)
-
-(** **** Exercise: 4 stars, optional (factorial_dec)  *)
-(** Remember the factorial function we worked with before: *)
-
-Fixpoint real_fact (n:nat) : nat :=
-  match n with
-  | O => 1
-  | S n' => n * (real_fact n')
-  end.
-
-(** Following the pattern of [subtract_slowly_dec], write a decorated
-    Imp program that implements the factorial function, and prove it
-    correct. *)
-
-(* FILL IN HERE *)
-(** [] *)
-
-
-(* $Date: 2013-03-11 14:56:33 -0400 (Mon, 11 Mar 2013) $ *)
+(** $Date: 2014-12-31 11:17:56 -0500 (Wed, 31 Dec 2014) $ *)
 
