Smallstep.v
@@ -1,44 +1,54 @@
 (** * Smallstep: Small-step Operational Semantics *)
 
-(* $Date: 2012-12-26 11:12:50 -1000 (Wed, 26 Dec 2012) $ *)
-
 Require Export Imp.
 
-(** The evaluators we have seen so far (e.g., the ones for [aexp]s,
-    [bexp]s, and commands) have been formulated in a "big-step"
-    style -- they specify how a given expression can be evaluated to
-    its final value (or a command plus a store to a final store) "all
-    in one big step."
+
+(** The evaluators we have seen so far (e.g., the ones for
+    [aexp]s, [bexp]s, and commands) have been formulated in a
+    "big-step" style -- they specify how a given expression can be
+    evaluated to its final value (or a command plus a store to a final
+    store) "all in one big step."
  
-    This style is simple and natural for many purposes (indeed, Gilles
-    Kahn, who popularized its use, called it _natural semantics_), but
-    there are some things it does not do well.  In particular, it
-    does not give us a natural way of talking about _concurrent_
-    programming languages, where the "semantics" of a program -- i.e.,
-    the essence of how it behaves -- is not just which input states
-    get mapped to which output states, but also includes the
-    intermediate states that it passes through along the way, since
-    these states can also be observed by concurrently executing code.
+    This style is simple and natural for many purposes -- indeed,
+    Gilles Kahn, who popularized its use, called it _natural
+    semantics_.  But there are some things it does not do well.  In
+    particular, it does not give us a natural way of talking about
+    _concurrent_ programming languages, where the "semantics" of a
+    program -- i.e., the essence of how it behaves -- is not just
+    which input states get mapped to which output states, but also
+    includes the intermediate states that it passes through along the
+    way, since these states can also be observed by concurrently
+    executing code.
 
     Another shortcoming of the big-step style is more technical, but
-    critical for some applications.  Consider the variant of Imp with
-    lists that we introduced in the [HoareList] chapter.  We chose to
-    define the meaning of programs like [0 + nil] by specifying that a
-    list should be interpreted as [0] when it occurs in a context
-    expecting a number, but this was a bit of a hack.  It would be
-    better simply to say that the behavior of such a program is
-    _undefined_ -- it doesn't evaluate to any result.  We could easily
-    do this: we'd just have to use the formulations of [aeval] and
-    [beval] as inductive propositions (rather than Fixpoints), so that
-    we can make them partial functions instead of total ones.
+    critical in some situations.  To see the issue, suppose we wanted
+    to define a variant of Imp where variables could hold _either_
+    numbers _or_ lists of numbers (see the [HoareList] chapter for
+    details).  In the syntax of this extended language, it will be
+    possible to write strange expressions like [2 + nil], and our
+    semantics for arithmetic expressions will then need to say
+    something about how such expressions behave.  One
+    possibility (explored in the [HoareList] chapter) is to maintain
+    the convention that every arithmetic expressions evaluates to some
+    number by choosing some way of viewing a list as a number -- e.g.,
+    by specifying that a list should be interpreted as [0] when it
+    occurs in a context expecting a number.  But this is really a bit
+    of a hack.
 
-    However, this way of defining Imp has a serious deficiency.  In
-    this language, a command might _fail_ to map a given starting
-    state to any ending state for two quite different reasons: either
-    because the execution gets into an infinite loop or because, at
-    some point, the program tries to do an operation that makes no
-    sense, such as taking the successor of a boolean variable, and
-    none of the evaluation rules can be applied.
+    A much more natural approach is simply to say that the behavior of
+    an expression like [2+nil] is _undefined_ -- it doesn't evaluate
+    to any result at all.  And we can easily do this: we just have to
+    formulate [aeval] and [beval] as [Inductive] propositions rather
+    than Fixpoints, so that we can make them partial functions instead
+    of total ones.
+
+    However, now we encounter a serious deficiency.  In this language,
+    a command might _fail_ to map a given starting state to any ending
+    state for two quite different reasons: either because the
+    execution gets into an infinite loop or because, at some point,
+    the program tries to do an operation that makes no sense, such as
+    adding a number to a list, and none of the evaluation rules can be
+    applied.
  
     These two outcomes -- nontermination vs. getting stuck in an
     erroneous configuration -- are quite different.  In particular, we
@@ -57,24 +67,6 @@ Require Export Imp.
     with a "small-step" relation that specifies, for a given program,
     how the "atomic steps" of computation are performed. *)
 
-(* ########################################################### *)
-(** * Relations *)
-
-(** A _relation_ on a set [X] is a family of propositions
-    parameterized by two elements of [X] -- i.e., a proposition about
-    pairs of elements of [X].  *)
-
-Definition relation (X: Type) := X->X->Prop.
-
-(** Our main examples of such relations in this chapter will be
-    the single-step and multi-step reduction relations on terms, [==>]
-    and [==>*], but there are many other examples -- some that come to
-    mind are the "equals," "less than," "less than or equal to," and
-    "is the square of" relations on numbers, and the "prefix of"
-    relation on lists and strings.
-
-    The optional [Rel] chapter tells a more detailed story about how
-    relations are treated in Coq. *)
 
 (* ########################################################### *)
 (** * A Toy Language *)
@@ -86,25 +78,21 @@ Definition relation (X: Type) := X->X->Prop.
     see how to apply the same techniques to the full Imp language.  *)
 
 Inductive tm : Type :=
-  | C : nat -> tm
-  | P : tm -> tm -> tm.
+  | C : nat -> tm         (* Constant *)
+  | P : tm -> tm -> tm.   (* Plus *)
 
 Tactic Notation "tm_cases" tactic(first) ident(c) :=
   first;
   [ Case_aux c "C" | Case_aux c "P" ].
 
-Module SimpleArith0.
-
 (** Here is a standard evaluator for this language, written in the
     same (big-step) style as we've been using up to this point. *)
 
-Fixpoint eval (t : tm) : nat :=
+Fixpoint evalF (t : tm) : nat :=
   match t with
   | C n => n
-  | P a1 a2 => eval a1 + eval a2
+  | P a1 a2 => evalF a1 + evalF a2
   end.
-
-End SimpleArith0.
 
 (** Now, here is the same evaluator, written in exactly the same
     style, but formulated as an inductively defined relation.  Again,
@@ -151,6 +139,8 @@ Module SimpleArith1.
                       P (C n1) t2 ==> P (C n1) t2'
 *)
 
+
+
 Reserved Notation " t '==>' t' " (at level 40).
 
 Inductive step : tm -> tm -> Prop :=
@@ -182,11 +172,12 @@ Tactic Notation "step_cases" tactic(first) ident(c) :=
 
     - A term that is just a constant cannot take a step. *)
 
-(** A couple of examples of reasoning with the [step]
-    relation... *)
+
+(** Let's pause and check a couple of examples of reasoning with
+    the [step] relation... *)
 
 (** If [t1] can take a step to [t1'], then [P t1 t2] steps
-    to [plus t1' t2]: *)
+    to [P t1' t2]: *)
 
 Example test_step_1 : 
       P 
@@ -199,7 +190,7 @@ Example test_step_1 :
 Proof.
   apply ST_Plus1. apply ST_PlusConstConst.  Qed.
 
-(** **** Exercise: 2 stars (test_step_2) *)
+(** **** Exercise: 1 star (test_step_2)  *)
 (** Right-hand sides of sums can take a step only when the
     left-hand side is finished: if [t2] can take a step to [t2'],
     then [P (C n) t2] steps to [P (C n)
@@ -221,15 +212,42 @@ Proof.
   (* FILL IN HERE *) Admitted.
 (** [] *)
 
+
+
+
+(* ########################################################### *)
+(** * Relations *)
+
+(** We will be using several different step relations, so it is
+    helpful to generalize a bit and state a few definitions and
+    theorems about relations in general.  (The optional chapter
+    [Rel.v] develops some of these ideas in a bit more detail; it may
+    be useful if the treatment here is too dense.) *)
+
+(** A (binary) _relation_ on a set [X] is a family of propositions
+    parameterized by two elements of [X] -- i.e., a proposition about
+    pairs of elements of [X].  *)
+
+Definition relation (X: Type) := X->X->Prop.
+
+
+(** Our main examples of such relations in this chapter will be
+    the single-step and multi-step reduction relations on terms, [==>]
+    and [==>*], but there are many other examples -- some that come to
+    mind are the "equals," "less than," "less than or equal to," and
+    "is the square of" relations on numbers, and the "prefix of"
+    relation on lists and strings. *)
+
+
 (** One simple property of the [==>] relation is that, like the
     evaluation relation for our language of Imp programs, it is
     _deterministic_.
 
     _Theorem_: For each [t], there is at most one [t'] such that [t]
     steps to [t'] ([t ==> t'] is provable).  Formally, this is the
-    same as saying that [==>] is deterministic.
+    same as saying that [==>] is deterministic. *)
 
-    _Proof sketch_: We show that if [x] steps to both [y1] and [y2]
+(** _Proof sketch_: We show that if [x] steps to both [y1] and [y2]
     then [y1] and [y2] are equal, by induction on a derivation of
     [step x y1].  There are several cases to consider, depending on
     the last rule used in this derivation and in the given derivation
@@ -275,7 +293,39 @@ Proof.
       SCase "ST_Plus1". inversion H2.
       SCase "ST_Plus2".
         rewrite <- (IHHy1 t2'0).
-        reflexivity. assumption.  Qed.
+        reflexivity. assumption.  
+Qed.
+
+(** There is some annoying repetition in this proof.
+    Each use of [inversion Hy2] results in three subcases, 
+    only one of which is relevant (the one which matches the 
+    current case in the induction on [Hy1]). The other two
+    subcases need to be dismissed by finding the contradiction
+    among the hypotheses and doing inversion on it.
+
+    There is a tactic called [solve by inversion] defined in [SfLib.v]
+    that can be of use in such cases. It will solve the goal if it
+    can be solved by inverting some hypothesis; otherwise, it fails.
+    (There are variants [solve by inversion 2] and [solve by inversion 3]
+    that work if two or three consecutive inversions will solve the goal.)
+
+    The example below shows how a proof of the previous theorem can be
+    simplified using this tactic.
+*)
+
+Theorem step_deterministic_alt: deterministic step.
+Proof.
+  intros x y1 y2 Hy1 Hy2.
+  generalize dependent y2.
+  step_cases (induction Hy1) Case; intros y2 Hy2; 
+    inversion Hy2; subst; try (solve by inversion).
+  Case "ST_PlusConstConst". reflexivity.
+  Case "ST_Plus1". 
+    apply IHHy1 in H2. rewrite H2. reflexivity.
+  Case "ST_Plus2".
+    apply IHHy1 in H2. rewrite H2. reflexivity.
+Qed.
+
 
 End SimpleArith1.
 
@@ -295,7 +345,8 @@ End SimpleArith1.
 
       - The _halting states_ of the machine are ones where there is no
         more computation to be done.
-
+*)
+(**
     We can then execute a term [t] as follows:
 
       - Take [t] as the starting state of the machine.
@@ -317,6 +368,7 @@ Inductive value : tm -> Prop :=
 (** Having introduced the idea of values, we can use it in the
     definition of the [==>] relation to write [ST_Plus2] rule in a
     slightly more elegant way: *)
+
 (** 
                      -------------------------------        (ST_PlusConstConst)
                      P (C n1) (C n2) ==> C (n1 + n2)
@@ -337,6 +389,8 @@ Inductive value : tm -> Prop :=
     to maintain a close correspondence between the informal and Coq
     versions of the rules, but later on we'll drop it in informal
     rules, for the sake of brevity.) *)
+
+(**  Here are the formal rules: *)
 
 Reserved Notation " t '==>' t' " (at level 40).
 
@@ -359,7 +413,7 @@ Tactic Notation "step_cases" tactic(first) ident(c) :=
   [ Case_aux c "ST_PlusConstConst"
   | Case_aux c "ST_Plus1" | Case_aux c "ST_Plus2" ].
 
-(** **** Exercise: 3 stars, recommended (redo_determinism) *)
+(** **** Exercise: 3 stars (redo_determinism)  *)
 (** As a sanity check on this change, let's re-verify determinism 
 
     Proof sketch: We must show that if [x] steps to both [y1] and [y2]
@@ -386,7 +440,6 @@ Tactic Notation "step_cases" tactic(first) ident(c) :=
     maximum benefit from the exercise you should try to write it from
     scratch and just use the earlier one if you get stuck. *)
 
-(** **** Exercise: 2 stars, optional (step_deterministic) *)
 Theorem step_deterministic :
   deterministic step.
 Proof.
@@ -403,10 +456,10 @@ Proof.
     to a value.  The following theorem shows that we did not, in fact,
     make such a mistake here. *)
 
-(** _Theorem_ (_Strong Progress_): For all [t:tm], either [t] is a
-    value, or there exists a term [t'] such that [t ==> t'].
+(** _Theorem_ (_Strong Progress_): If [t] is a term, then either [t]
+    is a value, or there exists a term [t'] such that [t ==> t']. *)
 
-    _Proof_: By induction on [t].
+(** _Proof_: By induction on [t].
 
     - Suppose [t = C n]. Then [t] is a [value].
 
@@ -448,9 +501,11 @@ Proof.
 
 (** The idea of "making progress" can be extended to tell us something
     interesting about [value]s: in this language [value]s are exactly
-    the terms that _cannot_ make progress in this sense.  To state
-    this fact, let's begin by giving a name to terms that cannot make
-    progress: We'll call them _normal forms_. *)
+    the terms that _cannot_ make progress in this sense.  
+
+    To state this observation formally, let's begin by giving a name
+    to terms that cannot make progress.  We'll call them _normal
+    forms_. *)
 
 Definition normal_form {X:Type} (R:relation X) (t:X) : Prop :=
   ~ exists t', R t t'.
@@ -466,10 +521,10 @@ Definition normal_form {X:Type} (R:relation X) (t:X) : Prop :=
     in the strong progress theorem: in this language, normal forms and
     values are actually the same thing. *)
 
-Lemma value_is_nf : forall t,
-  value t -> normal_form step t.
+Lemma value_is_nf : forall v,
+  value v -> normal_form step v.
 Proof.
-  unfold normal_form. intros t H. inversion H.
+  unfold normal_form. intros v H. inversion H.
   intros contra. inversion contra. inversion H1.
 Qed.
 
@@ -488,18 +543,16 @@ Corollary nf_same_as_value : forall t,
 Proof.
   split. apply nf_is_value. apply value_is_nf. Qed.
 
-(** Why is this interesting?  For two reasons:
- 
-    - Because [value] is a syntactic concept -- it is a defined by
-      looking at the form of a term -- while [normal_form] is a
-      semantic one -- it is defined by looking at how the term steps.
-      It is not obvious that these concepts should coincide!
- 
-    - Indeed, there are lots of languages in which the concepts of
-      normal form and value do _not_ coincide. *)
- 
-(** Let's examine how this can happen... *)
+(** Why is this interesting?  
 
+    Because [value] is a syntactic concept -- it is defined by looking
+    at the form of a term -- while [normal_form] is a semantic one --
+    it is defined by looking at how the term steps.  It is not obvious
+    that these concepts should coincide!
+ 
+    Indeed, we could easily have written the definitions so that they
+    would not coincide... *)
+ 
 (* ##################################################### *)
 
 (** We might, for example, mistakenly define [value] so that it
@@ -528,16 +581,17 @@ Inductive step : tm -> tm -> Prop :=
 
   where " t '==>' t' " := (step t t').
 
-(** **** Exercise: 3 stars, optional (value_not_same_as_normal_form) *)
+
+
+(** **** Exercise: 3 stars, advanced (value_not_same_as_normal_form)  *)
 Lemma value_not_same_as_normal_form :
-  exists t, value t /\ ~ normal_form step t.
+  exists v, value v /\ ~ normal_form step v.
 Proof.
   (* FILL IN HERE *) Admitted.
 (** [] *)
-
 End Temp1.
 
-(* ########################################################### *)
+(* ##################################################### *)
 (** Alternatively, we might mistakenly define [step] so that it
     permits something designated as a value to reduce further. *)
 
@@ -563,13 +617,14 @@ Inductive step : tm -> tm -> Prop :=
 
   where " t '==>' t' " := (step t t').
 
-(** **** Exercise: 2 stars, optional (value_not_same_as_normal_form) *)
+
+(** **** Exercise: 2 stars, advanced (value_not_same_as_normal_form)  *)
 Lemma value_not_same_as_normal_form :
-  exists t, value t /\ ~ normal_form step t.
+  exists v, value v /\ ~ normal_form step v.
 Proof.
   (* FILL IN HERE *) Admitted.
-(** [] *)
 
+(** [] *)
 End Temp2.
 
 (* ########################################################### *)
@@ -577,7 +632,7 @@ End Temp2.
     term that is not a value but that cannot take a step in the [step]
     relation.  Such terms are said to be _stuck_. In this case this is
     caused by a mistake in the semantics, but we will also see
-    situations where, evne in a correct language definition, it makes
+    situations where, even in a correct language definition, it makes
     sense to allow some terms to be stuck. *)
 
 Module Temp3.
@@ -598,7 +653,7 @@ Inductive step : tm -> tm -> Prop :=
 
 (** (Note that [ST_Plus2] is missing.) *)
 
-(** **** Exercise: 3 stars (value_not_same_as_normal_form') *)
+(** **** Exercise: 3 stars, advanced (value_not_same_as_normal_form')  *)
 Lemma value_not_same_as_normal_form :
   exists t, ~ value t /\ normal_form step t.
 Proof.
@@ -638,7 +693,7 @@ Inductive step : tm -> tm -> Prop :=
 
   where " t '==>' t' " := (step t t').
 
-(** **** Exercise: 1 star (smallstep_bools) *) 
+(** **** Exercise: 1 star (smallstep_bools)  *) 
 (** Which of the following propositions are provable?  (This is just a
     thought exercise, but for an extra challenge feel free to prove
     your answers in Coq.) *)
@@ -672,7 +727,7 @@ Definition bool_step_prop3 :=
 (* FILL IN HERE *)
 (** [] *)
 
-(** **** Exercise: 3 stars, recommended (progress_bool) *)
+(** **** Exercise: 3 stars, optional (progress_bool)  *)
 (** Just as we proved a progress theorem for plus expressions, we can
     do so for boolean expressions, as well. *)
 
@@ -682,7 +737,7 @@ Proof.
   (* FILL IN HERE *) Admitted.
 (** [] *)
 
-(** **** Exercise: 2 stars, optional (step_deterministic) *)
+(** **** Exercise: 2 stars, optional (step_deterministic)  *)
 Theorem step_deterministic :
   deterministic step.
 Proof.
@@ -691,7 +746,7 @@ Proof.
 
 Module Temp5. 
 
-(** **** Exercise: 2 stars (smallstep_bool_shortcut) *) 
+(** **** Exercise: 2 stars (smallstep_bool_shortcut)  *) 
 (** Suppose we want to add a "short circuit" to the step relation for
     boolean expressions, so that it can recognize when the [then] and
     [else] branches of a conditional are the same value (either
@@ -723,7 +778,6 @@ Inductive step : tm -> tm -> Prop :=
 (* FILL IN HERE *)
 
   where " t '==>' t' " := (step t t').
-(** [] *)
 
 Definition bool_step_prop4 :=
          tif
@@ -739,7 +793,7 @@ Proof.
   (* FILL IN HERE *) Admitted.
 (** [] *)
 
-(** **** Exercise: 3 stars, optional (properties_of_altered_step) *)
+(** **** Exercise: 3 stars, optional (properties_of_altered_step)  *)
 (** It can be shown that the determinism and strong progress theorems
     for the step relation in the lecture notes also hold for the
     definition of step given above.  After we add the clause
@@ -766,7 +820,7 @@ Proof.
      step relation? Write yes or no and briefly (1 sentence) explain
      your answer.
 
-  (* FILL IN HERE *)
+(* FILL IN HERE *)
 *)
 (** [] *)
 
@@ -792,12 +846,13 @@ End Temp4.
       [t] can reach by multi-step reduction. *)
 
 (* ########################################################### *)
-(** ** Definitions *)
 
 (** Since we'll want to reuse the idea of multi-step reduction many
     times in this and future chapters, let's take a little extra
-    trouble here and define it generically.  Given a relation [R], we
-    define a relation [multi R] as follows: *)
+    trouble here and define it generically.  
+
+    Given a relation [R], we define a relation [multi R], called the
+    _multi-step closure of [R]_ as follows: *)
 
 Inductive multi {X:Type} (R: relation X) : relation X :=
   | multi_refl  : forall (x : X), multi R x x
@@ -807,17 +862,42 @@ Inductive multi {X:Type} (R: relation X) : relation X :=
                     multi R x z.
 
 (** The effect of this definition is that [multi R] relates two
-    elements [x] and [y] of [X] if either [x = y] or else there is
-    some (possibly empty) sequence [z1], [z2], ..., [zn] such that:
-      R x z1
-      R z1 z2
-      ...
-      R zn y
+    elements [x] and [y] if either 
+
+       - [x = y], or else
+       - there is some sequence [z1], [z2], ..., [zn]
+         such that
+           R x z1
+           R z1 z2
+           ...
+           R zn y.
+
+    Thus, if [R] describes a single-step of computation, [z1],
+    ... [zn] is the sequence of intermediate steps of computation
+    between [x] and [y].
 *)
 
 Tactic Notation "multi_cases" tactic(first) ident(c) :=
   first;
   [ Case_aux c "multi_refl" | Case_aux c "multi_step" ].
+
+(** We write [==>*] for the [multi step] relation -- i.e., the
+    relation that relates two terms [t] and [t'] if we can get from
+    [t] to [t'] using the [step] relation zero or more times. *)
+
+Notation " t '==>*' t' " := (multi step t t') (at level 40).
+
+(** The relation [multi R] has several crucial properties.
+
+    First, it is obviously _reflexive_ (that is, [forall x, multi R x
+    x]).  In the case of the [==>*] (i.e. [multi step]) relation, the
+    intuition is that a term can execute to itself by taking zero
+    steps of execution.
+
+    Second, it contains [R] -- that is, single-step executions are a
+    particular case of multi-step executions.  (It is this fact that
+    justifies the word "closure" in the term "multi-step closure of
+    [R].") *)
 
 Theorem multi_R : forall (X:Type) (R:relation X) (x y : X),
        R x y -> (multi R) x y.
@@ -825,10 +905,7 @@ Proof.
   intros X R x y H.
   apply multi_step with y. apply H. apply multi_refl.   Qed.
 
-(** The crucial properties of the [multi R] relation are 
-       - [multi R] is reflexive
-       - [multi R] is transitive
-       - [multi R] relates everything related by [R] *)
+(** Third, [multi R] is _transitive_. *)
 
 Theorem multi_trans :
   forall (X:Type) (R: relation X) (x y z : X),
@@ -843,12 +920,7 @@ Proof.
       apply multi_step with y. assumption. 
       apply IHG. assumption.  Qed.
 
-(** We now write [==>*] for the [multi step] relation -- i.e., the
-    relation that relates two terms [t] and [t'] if we can get from
-    [t] to [t'] using the [step] relation zero or more times. *)
-
-Definition multistep := multi step.
-Notation " t '==>*' t' " := (multistep t t') (at level 40).
+(** That is, if [t1==>*t2] and [t2==>*t3], then [t1==>*t3]. *)
 
 (* ########################################################### *)
 (** ** Examples *)
@@ -890,14 +962,14 @@ Proof.
   eapply multi_step. apply ST_PlusConstConst.
   apply multi_refl.  Qed.
 
-(** **** Exercise: 1 star, optional (test_multistep_2) *)
+(** **** Exercise: 1 star, optional (test_multistep_2)  *)
 Lemma test_multistep_2:
   C 3 ==>* C 3.
 Proof.
   (* FILL IN HERE *) Admitted.
 (** [] *)
 
-(** **** Exercise: 1 star, optional (test_multistep_3) *)
+(** **** Exercise: 1 star, optional (test_multistep_3)  *)
 Lemma test_multistep_3:
       P (C 0) (C 3)
    ==>*
@@ -906,7 +978,7 @@ Proof.
   (* FILL IN HERE *) Admitted.
 (** [] *)
 
-(** **** Exercise: 2 stars (test_multistep_4) *)
+(** **** Exercise: 2 stars (test_multistep_4)  *)
 Lemma test_multistep_4:
       P
         (C 0)
@@ -939,7 +1011,7 @@ Definition normal_form_of (t t' : tm) :=
     can actually pronounce [normal_form t t'] as "[t'] is _the_
     normal form of [t]." *)
 
-(** **** Exercise: 3 stars, optional (normal_forms_unique) *)
+(** **** Exercise: 3 stars, optional (normal_forms_unique)  *)
 Theorem normal_forms_unique:
   deterministic normal_form_of.
 Proof.
@@ -978,7 +1050,7 @@ Proof.
         apply ST_Plus1. apply H. 
         apply IHmulti.  Qed.
 
-(** **** Exercise: 2 stars (multistep_congr_2) *)
+(** **** Exercise: 2 stars (multistep_congr_2)  *)
 Lemma multistep_congr_2 : forall t1 t2 t2',
      value t1 ->
      t2 ==>* t2' ->
@@ -1045,13 +1117,13 @@ Proof.
 (* ########################################################### *)
 (** ** Equivalence of Big-Step and Small-Step Reduction *)
 
-(** Having defined the operational semantics of our tiny
-    programming language in two different styles, it makes sense to
-    ask whether these definitions actually define the same thing!
-    They do, though it takes a little work to show it.  The details
-    are left to you. *)
+(** Having defined the operational semantics of our tiny programming
+    language in two different styles, it makes sense to ask whether
+    these definitions actually define the same thing!  They do, though
+    it takes a little work to show it.  (The details are left as an
+    exercise). *)
 
-(** **** Exercise: 3 stars (eval__multistep) *)
+(** **** Exercise: 3 stars (eval__multistep)  *)
 Theorem eval__multistep : forall t n,
   t || n -> t ==>* C n.
 
@@ -1075,9 +1147,9 @@ Theorem eval__multistep : forall t n,
          to a normal form, which must again be a term of the form [C
          n2] for some [n2].
        - Finally, we use [ST_PlusConstConst] one time to reduce [P (C
-         n1) (C n2)] to [C (n1 + n2)].
+         n1) (C n2)] to [C (n1 + n2)]. *)
 
-    To formalize this intuition, you'll need to use the congruence
+(** To formalize this intuition, you'll need to use the congruence
     lemmas from above (you might want to review them now, so that
     you'll be able to recognize when they are useful), plus some basic
     properties of [==>*]: that it is reflexive, transitive, and
@@ -1087,18 +1159,16 @@ Proof.
   (* FILL IN HERE *) Admitted.
 (** [] *)
 
-(** **** Exercise: 3 stars (eval__multistep_inf) *)
+(** **** Exercise: 3 stars, advanced (eval__multistep_inf)  *)
 (** Write a detailed informal version of the proof of [eval__multistep].
 
 (* FILL IN HERE *)
 []
 *)
+(** For the other direction, we need one lemma, which establishes a
+    relation between single-step reduction and big-step evaluation. *)
 
-(** For the other direction of the correspondence, we need one lemma,
-    which establishes a relation between single-step reduction and
-    big-step evaluation. *)
-
-(** **** Exercise: 3 stars (step__eval) *)
+(** **** Exercise: 3 stars (step__eval)  *)
 Lemma step__eval : forall t t' n,
      t ==> t' ->
      t' || n ->
@@ -1108,16 +1178,17 @@ Proof.
   (* FILL IN HERE *) Admitted.
 (** [] *)
 
-(** The main theorem is now straightforward to prove, once it is
-    stated correctly. The proof proceeds by induction on the
-    multipstep reduction sequence that is buried in the hypothesis
-    [normal_form_of t v]. *)
+(** The fact that small-step reduction implies big-step is now
+    straightforward to prove, once it is stated correctly. 
+
+    The proof proceeds by induction on the multi-step reduction
+    sequence that is buried in the hypothesis [normal_form_of t t']. *)
 (** Make sure you understand the statement before you start to
     work on the proof.  *)
 
-(** **** Exercise: 3 stars (multistep__eval) *)
-Theorem multistep__eval : forall t v,
-  normal_form_of t v -> exists n, v = C n /\ t || n.
+(** **** Exercise: 3 stars (multistep__eval)  *)
+Theorem multistep__eval : forall t t',
+  normal_form_of t t' -> exists n, t' = C n /\ t || n.
 Proof.
   (* FILL IN HERE *) Admitted.
 (** [] *)
@@ -1125,7 +1196,22 @@ Proof.
 (* ########################################################### *)
 (** ** Additional Exercises *)
 
-(** **** Exercise: 4 stars (combined_properties) *)
+(** **** Exercise: 3 stars, optional (interp_tm)  *)
+(** Remember that we also defined big-step evaluation of [tm]s as a
+    function [evalF].  Prove that it is equivalent to the existing
+    semantics.
+ 
+    Hint: we just proved that [eval] and [multistep] are
+    equivalent, so logically it doesn't matter which you choose.
+    One will be easier than the other, though!  *)
+
+Theorem evalF_eval : forall t n,
+  evalF t = n <-> t || n.
+Proof.
+  (* FILL IN HERE *) Admitted.
+(** [] *)
+
+(** **** Exercise: 4 stars (combined_properties)  *)
 (** We've considered the arithmetic and conditional expressions
     separately.  This exercise explores how the two interact. *)
 
@@ -1207,7 +1293,7 @@ Inductive aval : aexp -> Prop :=
   av_num : forall n, aval (ANum n).
 
 (** We are not actually going to bother to define boolean
-    values -- they aren't needed in the definition of [==>b]
+    values, since they aren't needed in the definition of [==>b]
     below (why?), though they might be if our language were a bit
     larger (why?). *)
 
@@ -1324,9 +1410,9 @@ Inductive cstep : (com * state) -> (com * state) -> Prop :=
       (i ::= (ANum n)) / st ==> SKIP / (update st i n)
   | CS_SeqStep : forall st c1 c1' st' c2,
       c1 / st ==> c1' / st' ->
-      (c1 ; c2) / st ==> (c1' ; c2) / st'
+      (c1 ;; c2) / st ==> (c1' ;; c2) / st'
   | CS_SeqFinish : forall st c2,
-      (SKIP ; c2) / st ==> c2 / st
+      (SKIP ;; c2) / st ==> c2 / st
   | CS_IfTrue : forall st c1 c2,
       IFB BTrue THEN c1 ELSE c2 FI / st ==> c1 / st
   | CS_IfFalse : forall st c1 c2,
@@ -1336,12 +1422,13 @@ Inductive cstep : (com * state) -> (com * state) -> Prop :=
       IFB b THEN c1 ELSE c2 FI / st ==> (IFB b' THEN c1 ELSE c2 FI) / st
   | CS_While : forall st b c1,
           (WHILE b DO c1 END) / st
-      ==> (IFB b THEN (c1; (WHILE b DO c1 END)) ELSE SKIP FI) / st
+      ==> (IFB b THEN (c1;; (WHILE b DO c1 END)) ELSE SKIP FI) / st
 
   where " t '/' st '==>' t' '/' st' " := (cstep (t,st) (t',st')).
 
+
 (* ########################################################### *)
-(** * Concurrent Imp (Optional) *)
+(** * Concurrent Imp *)
 
 (** Finally, to show the power of this definitional style, let's
     enrich Imp with a new form of command that runs two subcommands in
@@ -1368,14 +1455,14 @@ Tactic Notation "com_cases" tactic(first) ident(c) :=
 
 Notation "'SKIP'" := 
   CSkip.
-Notation "l '::=' a" := 
-  (CAss l a) (at level 60).
-Notation "c1 ; c2" := 
+Notation "x '::=' a" := 
+  (CAss x a) (at level 60).
+Notation "c1 ;; c2" := 
   (CSeq c1 c2) (at level 80, right associativity).
 Notation "'WHILE' b 'DO' c 'END'" := 
   (CWhile b c) (at level 80, right associativity).
-Notation "'IFB' e1 'THEN' e2 'ELSE' e3 'FI'" := 
-  (CIf e1 e2 e3) (at level 80, right associativity).
+Notation "'IFB' b 'THEN' c1 'ELSE' c2 'FI'" := 
+  (CIf b c1 c2) (at level 80, right associativity).
 Notation "'PAR' c1 'WITH' c2 'END'" := 
   (CPar c1 c2) (at level 80, right associativity).
 
@@ -1388,9 +1475,9 @@ Inductive cstep : (com * state)  -> (com * state) -> Prop :=
       (i ::= (ANum n)) / st ==> SKIP / (update st i n)
   | CS_SeqStep : forall st c1 c1' st' c2,
       c1 / st ==> c1' / st' ->
-      (c1 ; c2) / st ==> (c1' ; c2) / st'
+      (c1 ;; c2) / st ==> (c1' ;; c2) / st'
   | CS_SeqFinish : forall st c2,
-      (SKIP ; c2) / st ==> c2 / st
+      (SKIP ;; c2) / st ==> c2 / st
   | CS_IfTrue : forall st c1 c2,
       (IFB BTrue THEN c1 ELSE c2 FI) / st ==> c1 / st
   | CS_IfFalse : forall st c1 c2,
@@ -1400,7 +1487,7 @@ Inductive cstep : (com * state)  -> (com * state) -> Prop :=
       (IFB b THEN c1 ELSE c2 FI) / st ==> (IFB b' THEN c1 ELSE c2 FI) / st
   | CS_While : forall st b c1,
       (WHILE b DO c1 END) / st ==> 
-               (IFB b THEN (c1; (WHILE b DO c1 END)) ELSE SKIP FI) / st
+               (IFB b THEN (c1;; (WHILE b DO c1 END)) ELSE SKIP FI) / st
     (* New part: *)
   | CS_Par1 : forall st c1 c1' c2 st',
       c1 / st ==> c1' / st' -> 
@@ -1412,11 +1499,16 @@ Inductive cstep : (com * state)  -> (com * state) -> Prop :=
       (PAR SKIP WITH SKIP END) / st ==> SKIP / st
   where " t '/' st '==>' t' '/' st' " := (cstep (t,st) (t',st')).
 
+
 Definition cmultistep := multi cstep. 
 
 Notation " t '/' st '==>*' t' '/' st' " := 
    (multi cstep  (t,st) (t',st')) 
    (at level 40, st at level 39, t' at level 39).  
+
+
+
+
 
 (** Among the many interesting properties of this language is the fact
     that the following program can terminate with the variable [X] set
@@ -1501,20 +1593,22 @@ Proof.
 
 (** More generally... *)
 
-(** **** Exercise: 3 stars, optional *)
+(** **** Exercise: 3 stars, optional  *)
 Lemma par_body_n__Sn : forall n st,
   st X = n /\ st Y = 0 ->
   par_loop / st ==>* par_loop / (update st X (S n)).
 Proof.
   (* FILL IN HERE *) Admitted.
+(** [] *)
 
-(** **** Exercise: 3 stars, optional *)
+(** **** Exercise: 3 stars, optional  *)
 Lemma par_body_n : forall n st,
   st X = 0 /\ st Y = 0 ->
   exists st',
     par_loop / st ==>*  par_loop / st' /\ st' X = n /\ st' Y = 0.
 Proof.
   (* FILL IN HERE *) Admitted.
+(** [] *)
 
 (** ... the above loop can exit with [X] having any value
     whatsoever. *)
@@ -1542,8 +1636,58 @@ Proof.
   eapply multi_step. apply CS_ParDone.
   apply multi_refl.
 
-  rewrite update_neq. assumption. reflexivity.
+  rewrite update_neq. assumption. intro X; inversion X. 
 Qed.
 
 End CImp.
+
+(* ########################################################### *)
+(** * A Small-Step Stack Machine *)
+
+(** Last example: a small-step semantics for the stack machine example
+    from Imp.v. *)
+
+Definition stack := list nat.
+Definition prog  := list sinstr.
+
+Inductive stack_step : state -> prog * stack -> prog * stack -> Prop :=
+  | SS_Push : forall st stk n p',
+    stack_step st (SPush n :: p', stk)      (p', n :: stk)
+  | SS_Load : forall st stk i p',
+    stack_step st (SLoad i :: p', stk)      (p', st i :: stk)
+  | SS_Plus : forall st stk n m p',
+    stack_step st (SPlus :: p', n::m::stk)  (p', (m+n)::stk)
+  | SS_Minus : forall st stk n m p',
+    stack_step st (SMinus :: p', n::m::stk) (p', (m-n)::stk)
+  | SS_Mult : forall st stk n m p',
+    stack_step st (SMult :: p', n::m::stk)  (p', (m*n)::stk).
+
+Theorem stack_step_deterministic : forall st, 
+  deterministic (stack_step st).
+Proof.
+  unfold deterministic. intros st x y1 y2 H1 H2.
+  induction H1; inversion H2; reflexivity.
+Qed.
+
+Definition stack_multistep st := multi (stack_step st).
+
+(** **** Exercise: 3 stars, advanced (compiler_is_correct)  *)
+(** Remember the definition of [compile] for [aexp] given in the 
+    [Imp] chapter. We want now to prove [compile] correct with respect
+    to the stack machine.
+
+    State what it means for the compiler to be correct according to 
+    the stack machine small step semantics and then prove it. *)
+
+Definition compiler_is_correct_statement : Prop := 
+(* FILL IN HERE *) admit.
+
+
+Theorem compiler_is_correct : compiler_is_correct_statement.
+Proof.
+(* FILL IN HERE *) Admitted.
+(** [] *)
+
+(** $Date: 2014-12-31 15:16:58 -0500 (Wed, 31 Dec 2014) $ *)
+
 
