Sub.v
@@ -1,8 +1,7 @@
 (** * Sub: Subtyping *)
 
-(* $Date: 2012-07-17 12:18:15 -1000 (Tue, 17 Jul 2012) $ *)
 
-Require Export MoreStlc.
+Require Export Types.
 
 (* ###################################################### *)
 (** * Concepts *)
@@ -107,6 +106,16 @@ Require Export MoreStlc.
     concepts behind the subclass / subinterface relation in the
     simplified setting of the STLC. *)
 
+(** *** *)
+(** Of course, real OO languages have lots of other features...
+       - mutable fields
+       - [private] and other visibility modifiers
+       - method inheritance
+       - static components
+       - etc., etc.
+
+    We'll ignore all these and focus on core mechanisms. *)
+
 (** ** The Subsumption Rule *)
 
 (** Our goal for this chapter is to add subtyping to the simply typed
@@ -144,8 +153,8 @@ Require Export MoreStlc.
                               S <: U    U <: T
                               ----------------                        (S_Trans)
                                    S <: T
-    ... and a rule of _reflexivity_, since any type [T] is always just
-    as good as itself:
+    ... and a rule of _reflexivity_, since certainly any type [T] is 
+    as good as itself:  
                                    ------                              (S_Refl)
                                    T <: T
 *)
@@ -157,16 +166,14 @@ Require Export MoreStlc.
     than" another if each of its components is.
                             S1 <: T1    S2 <: T2
                             --------------------                        (S_Prod)
-                               S1*S2 <: T1*T2
+                             S1 * S2 <: T1 * T2
 *)
 
 (** *** Arrows *)
 
 (** Suppose we have two functions [f] and [g] with these types:
-<<
        f : C -> Student 
-       g : (C -> Person) -> D
->>
+       g : (C->Person) -> D
     That is, [f] is a function that yields a record of type [Student],
     and [g] is a (higher-order) function that expects its (function)
     argument to yield a record of type [Person].  Also suppose, even
@@ -185,12 +192,12 @@ Require Export MoreStlc.
     their results are:
                                   S2 <: T2
                               ----------------                     (S_Arrow_Co)
-                              S1->S2 <: S1->T2
+                            S1 -> S2 <: S1 -> T2
     We can generalize this to allow the arguments of the two arrow
     types to be in the subtype relation as well:
                             T1 <: S1    S2 <: T2
                             --------------------                      (S_Arrow)
-                              S1->S2 <: T1->T2
+                            S1 -> S2 <: T1 -> T2
     Notice that the argument types are subtypes "the other way round":
     in order to conclude that [S1->S2] to be a subtype of [T1->T2], it
     must be the case that [T1] is a subtype of [S1].  The arrow
@@ -198,10 +205,8 @@ Require Export MoreStlc.
     and _covariant_ in its second. 
 
     Here is an example that illustrates this: 
-<<
        f : Person -> C
        g : (Student -> C) -> D
->>
     The application [g f] is safe, because the only thing the body of
     [g] can do with [f] is to apply it to some argument of type
     [Student].  Since [f] requires records having (at least) the
@@ -218,59 +223,36 @@ Require Export MoreStlc.
     viewed as having type [T1->T2]. 
 *)
 
-(** **** Exercise: 2 stars, recommended (arrow_sub_wrong) *)
-(** Suppose we had incorrectly defined subtyping as covariant on both
-    the right and the left of arrow types:
-                            S1 <: T1    S2 <: T2
-                            --------------------                (S_Arrow_wrong)
-                              S1->S2 <: T1->T2
-    Give a concrete example of functions [f] and [g] with types...
-<<
-       f : Student -> Nat
-       g : (Person -> Nat) -> Nat
->>
-    ... such that the application [g f] will get stuck during
-    execution.
-
-[]
-*)
-
 (** *** Records *)
 
-(** What about subtyping for record types?  
+(** What about subtyping for record types? *)
 
-   The basic intuition about subtyping for record types is that it is
+(** The basic intuition about subtyping for record types is that it is
    always safe to use a "bigger" record in place of a "smaller" one.
    That is, given a record type, adding extra fields will always
    result in a subtype.  If some code is expecting a record with
    fields [x] and [y], it is perfectly safe for it to receive a record
    with fields [x], [y], and [z]; the [z] field will simply be ignored.
    For example,
-<<
        {name:String, age:Nat, gpa:Nat} <: {name:String, age:Nat}
        {name:String, age:Nat} <: {name:String}
        {name:String} <: {}
->>
-   This is known as "width subtyping" for records.
+   This is known as "width subtyping" for records. *)
 
-   We can also create a subtype of a record type by replacing the type
+(** We can also create a subtype of a record type by replacing the type
    of one of its fields with a subtype.  If some code is expecting a
    record with a field [x] of type [T], it will be happy with a record
    having a field [x] of type [S] as long as [S] is a subtype of
    [T]. For example,
-<<
        {x:Student} <: {x:Person}
->>
-   This is known as "depth subtyping".
+   This is known as "depth subtyping". *)
 
-   Finally, although the fields of a record type are written in a
+(** Finally, although the fields of a record type are written in a
    particular order, the order does not really matter. For example, 
-<<
        {name:String,age:Nat} <: {age:Nat,name:String}
->>
-   This is known as "permutation subtyping".
+   This is known as "permutation subtyping". *)
 
-   We could formalize these requirements in a single subtyping rule
+(** We could formalize these requirements in a single subtyping rule
    for records as follows:
                         for each jk in j1..jn,
                     exists ip in i1..im, such that
@@ -282,25 +264,25 @@ Require Export MoreStlc.
    common fields should be in the subtype relation. However, this rule
    is rather heavy and hard to read.  If we like, we can decompose it
    into three simpler rules, which can be combined using [S_Trans] to
-   achieve all the same effects.
+   achieve all the same effects. *)
 
-    First, adding fields to the end of a record type gives a subtype:
+(** First, adding fields to the end of a record type gives a subtype:
                                n > m
                  ---------------------------------                 (S_RcdWidth)
                  {i1:T1...in:Tn} <: {i1:T1...im:Tm} 
    We can use [S_RcdWidth] to drop later fields of a multi-field
    record while keeping earlier fields, showing for example that
-   [{age:Nat,name:String} <: {name:String,age:Nat}].
+   [{age:Nat,name:String} <: {name:String}]. *)
 
-   Second, we can apply subtyping inside the components of a compound
+(** Second, we can apply subtyping inside the components of a compound
    record type:
                        S1 <: T1  ...  Sn <: Tn
                   ----------------------------------               (S_RcdDepth)
                   {i1:S1...in:Sn} <: {i1:T1...in:Tn}
    For example, we can use [S_RcdDepth] and [S_RcdWidth] together to
-   show that [{y:Student, x:Nat} <: {y:Person}].
+   show that [{y:Student, x:Nat} <: {y:Person}]. *)
 
-   Third, we need to be able to reorder fields.  For example, we
+(** Third, we need to be able to reorder fields.  For example, we
    might expect that [{name:String, gpa:Nat, age:Nat} <: Person].  We
    haven't quite achieved this yet: using just [S_RcdDepth] and
    [S_RcdWidth] we can only drop fields from the _end_ of a record
@@ -327,6 +309,20 @@ Require Export MoreStlc.
     - A class may implement multiple interfaces -- so-called "multiple
       inheritance" of interfaces (i.e., permutation is allowed for
       interfaces). *)
+
+(** **** Exercise: 2 stars (arrow_sub_wrong)  *)
+(** Suppose we had incorrectly defined subtyping as covariant on both
+    the right and the left of arrow types:
+                            S1 <: T1    S2 <: T2
+                            --------------------                (S_Arrow_wrong)
+                            S1 -> S2 <: T1 -> T2
+    Give a concrete example of functions [f] and [g] with the following types...
+       f : Student -> Nat
+       g : (Person -> Nat) -> Nat
+    ... such that the application [g f] will get stuck during
+    execution.
+
+[] *)
 
 (** *** Top *)
 
@@ -367,11 +363,11 @@ Require Export MoreStlc.
 
                             S1 <: T1    S2 <: T2
                             --------------------                       (S_Prod)
-                               S1*S2 <: T1*T2
+                             S1 * S2 <: T1 * T2
 
                             T1 <: S1    S2 <: T2
                             --------------------                      (S_Arrow)
-                              S1->S2 <: T1->T2
+                            S1 -> S2 <: T1 -> T2
 
                                n > m
                  ---------------------------------                 (S_RcdWidth)
@@ -386,10 +382,12 @@ Require Export MoreStlc.
                   {i1:S1...in:Sn} <: {i1:T1...in:Tn}
 *)
 
+
+
 (* ############################################### *)
 (** ** Exercises *)
 
-(** **** Exercise: 1 star, optional (subtype_instances_tf_1) *)
+(** **** Exercise: 1 star, optional (subtype_instances_tf_1)  *)
 (** Suppose we have types [S], [T], [U], and [V] with [S <: T]
     and [U <: V].  Which of the following subtyping assertions
     are then true?  Write _true_ or _false_ after each one.  
@@ -409,10 +407,9 @@ Require Export MoreStlc.
 
     - [S*V <: T*U]
 
-[]
-*)
+[] *)
 
-(** **** Exercise: 2 stars (subtype_order) *)
+(** **** Exercise: 2 stars (subtype_order)  *)
 (** The following types happen to form a linear order with respect to subtyping:
     - [Top]
     - [Top -> Student]
@@ -428,7 +425,7 @@ Where does the type [Top->Top->Student] fit into this order?
 
 *)
 
-(** **** Exercise: 1 star (subtype_instances_tf_2) *)
+(** **** Exercise: 1 star (subtype_instances_tf_2)  *)
 (** Which of the following statements are true?  Write _true_ or
     _false_ after each one.
       forall S T,
@@ -440,7 +437,7 @@ Where does the type [Top->Top->Student] fit into this order?
            exists T,
               S = T->T  /\  T <: A
 
-      forall S T1 T1,
+      forall S T1 T2,
            (S <: T1 -> T2) ->
            exists S1 S2,
               S = S1 -> S2  /\  T1 <: S1  /\  S2 <: T2 
@@ -451,13 +448,13 @@ Where does the type [Top->Top->Student] fit into this order?
       exists S,
            S->S <: S   
 
-      forall S T2 T2,
+      forall S T1 T2,
            S <: T1*T2 ->
            exists S1 S2,
               S = S1*S2  /\  S1 <: T1  /\  S2 <: T2  
 [] *)
 
-(** **** Exercise: 1 star (subtype_concepts_tf) *)
+(** **** Exercise: 1 star (subtype_concepts_tf)  *)
 (** Which of the following statements are true, and which are false?
     - There exists a type that is a supertype of every other type.
 
@@ -485,10 +482,9 @@ Where does the type [Top->Top->Student] fit into this order?
       [S0], [S1], etc., such that all the [Si]'s are different and
       each [S(i+1)] is a supertype of [Si].
 
-[]
-*)
+[] *)
 
-(** **** Exercise: 2 stars (proper_subtypes) *)
+(** **** Exercise: 2 stars (proper_subtypes)  *)
 (** Is the following statement true or false?  Briefly explain your
     answer.
     forall T,
@@ -496,10 +492,9 @@ Where does the type [Top->Top->Student] fit into this order?
          exists S,
             S <: T  /\  S <> T
 ]] 
-[]
-*)
+[] *)
 
-(** **** Exercise: 2 stars (small_large_1) *)
+(** **** Exercise: 2 stars (small_large_1)  *)
 (** 
    - What is the _smallest_ type [T] ("smallest" in the subtype
      relation) that makes the following assertion true?  (Assume we
@@ -509,10 +504,9 @@ Where does the type [Top->Top->Student] fit into this order?
 
    - What is the _largest_ type [T] that makes the same assertion true?
 
-[]
-*)
+[] *)
 
-(** **** Exercise: 2 stars (small_large_2) *)
+(** **** Exercise: 2 stars (small_large_2)  *)
 (** 
    - What is the _smallest_ type [T] that makes the following
      assertion true?
@@ -520,10 +514,9 @@ Where does the type [Top->Top->Student] fit into this order?
 
    - What is the _largest_ type [T] that makes the same assertion true?
 
-[]
-*)
+[] *)
 
-(** **** Exercise: 2 stars, optional (small_large_3) *)
+(** **** Exercise: 2 stars, optional (small_large_3)  *)
 (** 
    - What is the _smallest_ type [T] that makes the following
      assertion true?
@@ -531,10 +524,12 @@ Where does the type [Top->Top->Student] fit into this order?
 
    - What is the _largest_ type [T] that makes the same assertion true?
 
-[]
-*)
+[] *)
 
-(** **** Exercise: 2 stars (small_large_4) *)
+
+
+
+(** **** Exercise: 2 stars (small_large_4)  *)
 (** 
    - What is the _smallest_ type [T] that makes the following
      assertion true?
@@ -544,27 +539,24 @@ Where does the type [Top->Top->Student] fit into this order?
    - What is the _largest_ type [T] that makes the same
      assertion true?
 
-[]
-*)
+[] *)
 
-(** **** Exercise: 2 stars (smallest_1) *)
+(** **** Exercise: 2 stars (smallest_1)  *)
 (** What is the _smallest_ type [T] that makes the following
     assertion true?
       exists S, exists t, 
         empty |- (\x:T. x x) t : S
 ]] 
-[]
-*)
+[] *)
 
-(** **** Exercise: 2 stars (smallest_2) *)
+(** **** Exercise: 2 stars (smallest_2)  *)
 (** What is the _smallest_ type [T] that makes the following
     assertion true?
       empty |- (\x:Top. x) ((\z:A.z) , (\z:B.z)) : T
 ]] 
-[]
-*)
+[] *)
 
-(** **** Exercise: 3 stars, optional (count_supertypes) *)
+(** **** Exercise: 3 stars, optional (count_supertypes)  *)
 (** How many supertypes does the record type [{x:A, y:C->C}] have?  That is,
     how many different types [T] are there such that [{x:A, y:C->C} <:
     T]?  (We consider two types to be different if they are written
@@ -572,10 +564,9 @@ Where does the type [Top->Top->Student] fit into this order?
     [{x:A,y:B}] and [{y:B,x:A}] are different.)
 
 
-[]
-*)
+[] *)
 
-(** **** Exercise: 2 stars (pair_permutation) *)
+(** **** Exercise: 2 stars (pair_permutation)  *)
 (** The subtyping rule for product types
                             S1 <: T1    S2 <: T2
                             --------------------                        (S_Prod)
@@ -586,8 +577,7 @@ intuitively corresponds to the "depth" subtyping rule for records. Extending the
 for products.
 Is this a good idea? Briefly explain why or why not.
 
-[]
-*)
+[] *)
 
 (* ###################################################### *)
 (** * Formal Definitions *)
@@ -650,15 +640,15 @@ Tactic Notation "t_cases" tactic(first) ident(c) :=
 (* ################################### *)
 (** *** Substitution *)
 
-(** The definition of substitution remains the same as for the
-    ordinary STLC. *)
+(** The definition of substitution remains exactly the same as for the
+    pure STLC. *)
 
 Fixpoint subst (x:id) (s:tm)  (t:tm) : tm :=
   match t with
   | tvar y => 
-      if beq_id x y then s else t
+      if eq_id_dec x y then s else t
   | tabs y T t1 => 
-      tabs y T (if beq_id x y then t1 else (subst x s t1))
+      tabs y T (if eq_id_dec x y then t1 else (subst x s t1))
   | tapp t1 t2 => 
       tapp (subst x s t1) (subst x s t2)
   | ttrue => 
@@ -682,9 +672,9 @@ Notation "'[' x ':=' s ']' t" := (subst x s t) (at level 20).
 Inductive value : tm -> Prop :=
   | v_abs : forall x T t,
       value (tabs x T t)
-  | t_true : 
+  | v_true : 
       value ttrue
-  | t_false : 
+  | v_false : 
       value tfalse
   | v_unit : 
       value tunit
@@ -733,20 +723,22 @@ Hint Constructors step.
 (** The definition of subtyping is just what we sketched in the
     motivating discussion. *)
 
+Reserved Notation "T '<:' U" (at level 40).
+
 Inductive subtype : ty -> ty -> Prop :=
   | S_Refl : forall T,
-    subtype T T
+      T <: T
   | S_Trans : forall S U T,
-    subtype S U ->
-    subtype U T ->
-    subtype S T
+      S <: U ->
+      U <: T ->
+      S <: T
   | S_Top : forall S,
-    subtype S TTop
+      S <: TTop
   | S_Arrow : forall S1 S2 T1 T2,
-    subtype T1 S1 ->
-    subtype S2 T2 ->
-    subtype (TArrow S1 S2) (TArrow T1 T2)
-.
+      T1 <: S1 ->
+      S2 <: T2 ->
+      (TArrow S1 S2) <: (TArrow T1 T2)
+where "T '<:' U" := (subtype T U).
 
 (** Note that we don't need any special rules for base types: they are
     automatically subtypes of themselves (by [S_Refl]) and [Top] (by
@@ -774,7 +766,7 @@ Notation String := (TBase (Id 9)).
 Notation Float := (TBase (Id 10)).
 Notation Integer := (TBase (Id 11)).
 
-(** **** Exercise: 2 stars, optional (subtyping_judgements) *)
+(** **** Exercise: 2 stars, optional (subtyping_judgements)  *)
 
 (** (Do this exercise after you have added product types to the
     language, at least up to this point in the file).
@@ -786,6 +778,10 @@ Notation Integer := (TBase (Id 11)).
                   gpa  : Float }
     Employee := { name : String ;
                   ssn  : Integer }
+
+Recall that in chapter MoreStlc, the optional subsection "Encoding
+Records" describes how records can be encoded as pairs.
+
 *)
 
 Definition Person : ty := 
@@ -796,20 +792,19 @@ Definition Employee : ty :=
 (* FILL IN HERE *) admit.
 
 Example sub_student_person :
-  subtype Student Person.
+  Student <: Person.
 Proof. 
 (* FILL IN HERE *) Admitted.
 
 Example sub_employee_person :
-  subtype Employee Person.
+  Employee <: Person.
 Proof. 
 (* FILL IN HERE *) Admitted.
 (** [] *)
 
 Example subtyping_example_0 :
-  subtype (TArrow C Person) 
-          (TArrow C TTop).
-(* C->Person <: C->Top *)
+  (TArrow C Person) <: (TArrow C TTop).
+  (* C->Person <: C->Top *)
 Proof.
   apply S_Arrow.
     apply S_Refl. auto.
@@ -819,20 +814,18 @@ Qed.
     full benefit from the exercises, make sure you also
     understand how to prove them on paper! *)
 
-(** **** Exercise: 1 star, optional (subtyping_example_1) *)
+(** **** Exercise: 1 star, optional (subtyping_example_1)  *)
 Example subtyping_example_1 :
-  subtype (TArrow TTop Student) 
-          (TArrow (TArrow C C) Person).
-(* Top->Student <: (C->C)->Person *)
+  (TArrow TTop Student) <: (TArrow (TArrow C C) Person).
+  (* Top->Student <: (C->C)->Person *)
 Proof with eauto.
   (* FILL IN HERE *) Admitted.
 (** [] *)
 
-(** **** Exercise: 1 star, optional (subtyping_example_2) *)
+(** **** Exercise: 1 star, optional (subtyping_example_2)  *)
 Example subtyping_example_2 :
-  subtype (TArrow TTop Person) 
-          (TArrow Person TTop).
-(* Top->Person <: Person->Top *)
+  (TArrow TTop Person) <: (TArrow Person TTop).
+  (* Top->Person <: Person->Top *)
 Proof with eauto.
   (* FILL IN HERE *) Admitted.
 (** [] *)
@@ -849,36 +842,40 @@ End Examples.
 Definition context := id -> (option ty).
 Definition empty : context := (fun _ => None). 
 Definition extend (Gamma : context) (x:id) (T : ty) :=
-  fun x' => if beq_id x x' then Some T else Gamma x'.
+  fun x' => if eq_id_dec x x' then Some T else Gamma x'.
+
+Reserved Notation "Gamma '|-' t '\in' T" (at level 40).
 
 Inductive has_type : context -> tm -> ty -> Prop :=
   (* Same as before *)
   | T_Var : forall Gamma x T,
       Gamma x = Some T ->
-      has_type Gamma (tvar x) T
+      Gamma |- (tvar x) \in T
   | T_Abs : forall Gamma x T11 T12 t12,
-      has_type (extend Gamma x T11) t12 T12 -> 
-      has_type Gamma (tabs x T11 t12) (TArrow T11 T12)
+      (extend Gamma x T11) |- t12 \in T12 -> 
+      Gamma |- (tabs x T11 t12) \in (TArrow T11 T12)
   | T_App : forall T1 T2 Gamma t1 t2,
-      has_type Gamma t1 (TArrow T1 T2) -> 
-      has_type Gamma t2 T1 -> 
-      has_type Gamma (tapp t1 t2) T2
+      Gamma |- t1 \in (TArrow T1 T2) -> 
+      Gamma |- t2 \in T1 -> 
+      Gamma |- (tapp t1 t2) \in T2
   | T_True : forall Gamma,
-       has_type Gamma ttrue TBool
+       Gamma |- ttrue \in TBool
   | T_False : forall Gamma,
-       has_type Gamma tfalse TBool
+       Gamma |- tfalse \in TBool
   | T_If : forall t1 t2 t3 T Gamma,
-       has_type Gamma t1 TBool ->
-       has_type Gamma t2 T ->
-       has_type Gamma t3 T ->
-       has_type Gamma (tif t1 t2 t3) T
+       Gamma |- t1 \in TBool ->
+       Gamma |- t2 \in T ->
+       Gamma |- t3 \in T ->
+       Gamma |- (tif t1 t2 t3) \in T
   | T_Unit : forall Gamma,
-      has_type Gamma tunit TUnit
+      Gamma |- tunit \in TUnit
   (* New rule of subsumption *)
   | T_Sub : forall Gamma t S T,
-      has_type Gamma t S ->
-      subtype S T ->
-      has_type Gamma t T.
+      Gamma |- t \in S ->
+      S <: T ->
+      Gamma |- t \in T
+
+where "Gamma '|-' t '\in' T" := (has_type Gamma t T).
 
 Hint Constructors has_type.
 
@@ -890,6 +887,13 @@ Tactic Notation "has_type_cases" tactic(first) ident(c) :=
   | Case_aux c "T_Unit"     
   | Case_aux c "T_Sub" ].
 
+(* To make your job simpler, the following hints help construct typing
+   derivations. *)
+Hint Extern 2 (has_type _ (tapp _ _) _) => 
+  eapply T_App; auto.
+Hint Extern 2 (_ = _) => compute; reflexivity.
+
+
 (* ############################################### *)
 (** ** Typing examples *)
 
@@ -900,19 +904,19 @@ Import Examples.
     the language.  For each informal typing judgement, write it as a
     formal statement in Coq and prove it. *)
 
-(** **** Exercise: 1 star, optional (typing_example_0) *)
+(** **** Exercise: 1 star, optional (typing_example_0)  *)
 (* empty |- ((\z:A.z), (\z:B.z)) 
           : (A->A * B->B) *)
 (* FILL IN HERE *)
 (** [] *)
 
-(** **** Exercise: 2 stars, optional (typing_example_1) *)
+(** **** Exercise: 2 stars, optional (typing_example_1)  *)
 (* empty |- (\x:(Top * B->B). x.snd) ((\z:A.z), (\z:B.z)) 
           : B->B *)
 (* FILL IN HERE *)
 (** [] *)
 
-(** **** Exercise: 2 stars, optional (typing_example_2) *)
+(** **** Exercise: 2 stars, optional (typing_example_2)  *)
 (* empty |- (\z:(C->C)->(Top * B->B). (z (\x:C.x)).snd)
               (\z:C->C. ((\z:A.z), (\z:B.z)))
           : B->B *)
@@ -937,7 +941,7 @@ End Examples2.
     to record a couple of critical structural properties of the subtype
     relation: 
        - [Bool] is the only subtype of [Bool]
-       - every subtype of an arrow type _is_ an arrow type. *)
+       - every subtype of an arrow type is itself an arrow type. *)
     
 (** These are called _inversion lemmas_ because they play the same
     role in later proofs as the built-in [inversion] tactic: given a
@@ -947,20 +951,20 @@ End Examples2.
     tell us something further about the shapes of [S] and [T] and the
     existence of subtype relations between their parts. *)
 
-(** **** Exercise: 2 stars, optional (sub_inversion_Bool) *)
+(** **** Exercise: 2 stars, optional (sub_inversion_Bool)  *)
 Lemma sub_inversion_Bool : forall U,
-     subtype U TBool ->
+     U <: TBool ->
        U = TBool.
 Proof with auto.
   intros U Hs.
   remember TBool as V.
   (* FILL IN HERE *) Admitted.
 
-(** **** Exercise: 3 stars, optional (sub_inversion_arrow) *)
+(** **** Exercise: 3 stars, optional (sub_inversion_arrow)  *)
 Lemma sub_inversion_arrow : forall U V1 V2,
-     subtype U (TArrow V1 V2) ->
+     U <: (TArrow V1 V2) ->
      exists U1, exists U2, 
-       U = (TArrow U1 U2) /\ (subtype V1 U1) /\ (subtype U2 V2).
+       U = (TArrow U1 U2) /\ (V1 <: U1) /\ (U2 <: V2).
 Proof with eauto.
   intros U V1 V2 Hs.
   remember (TArrow V1 V2) as V.
@@ -996,9 +1000,9 @@ Proof with eauto.
     tells us the possible "canonical forms" (i.e. values) of function
     type. *)
 
-(** **** Exercise: 3 stars, optional (canonical_forms_of_arrow_types) *)
+(** **** Exercise: 3 stars, optional (canonical_forms_of_arrow_types)  *)
 Lemma canonical_forms_of_arrow_types : forall Gamma s T1 T2,
-  has_type Gamma s (TArrow T1 T2) ->
+  Gamma |- s \in (TArrow T1 T2) ->
   value s ->
   exists x, exists S1, exists s2,
      s = tabs x S1 s2.
@@ -1010,7 +1014,7 @@ Proof with eauto.
     [true] and [false]. *)
 
 Lemma canonical_forms_of_Bool : forall Gamma s,
-  has_type Gamma s TBool ->
+  Gamma |- s \in TBool ->
   value s ->
   (s = ttrue \/ s = tfalse).
 Proof with eauto.
@@ -1080,7 +1084,7 @@ Qed.
 *)
 
 Theorem progress : forall t T, 
-     has_type empty t T ->
+     empty |- t \in T ->
      value t \/ exists t', t ==> t'. 
 Proof with eauto.
   intros t T Ht.
@@ -1155,9 +1159,9 @@ Qed.
        <: T] then follows by [S_Trans]. *)
 
 Lemma typing_inversion_abs : forall Gamma x S1 t2 T,
-     has_type Gamma (tabs x S1 t2) T ->
-     (exists S2, subtype (TArrow S1 S2) T
-              /\ has_type (extend Gamma x S1) t2 S2).
+     Gamma |- (tabs x S1 t2) \in T ->
+     (exists S2, (TArrow S1 S2) <: T
+              /\ (extend Gamma x S1) |- t2 \in S2).
 Proof with eauto.
   intros Gamma x S1 t2 T H.
   remember (tabs x S1 t2) as t.
@@ -1172,9 +1176,9 @@ Proof with eauto.
 (** Similarly... *)
 
 Lemma typing_inversion_var : forall Gamma x T,
-  has_type Gamma (tvar x) T ->
+  Gamma |- (tvar x) \in T ->
   exists S,
-    Gamma x = Some S /\ subtype S T.
+    Gamma x = Some S /\ S <: T.
 Proof with eauto.
   intros Gamma x T Hty.
   remember (tvar x) as t.
@@ -1186,10 +1190,10 @@ Proof with eauto.
     destruct IHHty as [U [Hctx HsubU]]... Qed.
 
 Lemma typing_inversion_app : forall Gamma t1 t2 T2,
-  has_type Gamma (tapp t1 t2) T2 ->
+  Gamma |- (tapp t1 t2) \in T2 ->
   exists T1,
-    has_type Gamma t1 (TArrow T1 T2) /\
-    has_type Gamma t2 T1.
+    Gamma |- t1 \in (TArrow T1 T2) /\
+    Gamma |- t2 \in T1.
 Proof with eauto.
   intros Gamma t1 t2 T2 Hty.
   remember (tapp t1 t2) as t.
@@ -1202,8 +1206,8 @@ Proof with eauto.
 Qed.
 
 Lemma typing_inversion_true : forall Gamma T,
-  has_type Gamma ttrue T ->
-  subtype TBool T.
+  Gamma |- ttrue \in T ->
+  TBool <: T.
 Proof with eauto.
   intros Gamma T Htyp. remember ttrue as tu.
   has_type_cases (induction Htyp) Case;
@@ -1211,8 +1215,8 @@ Proof with eauto.
 Qed.
 
 Lemma typing_inversion_false : forall Gamma T,
-  has_type Gamma tfalse T ->
-  subtype TBool T.
+  Gamma |- tfalse \in T ->
+  TBool <: T.
 Proof with eauto.
   intros Gamma T Htyp. remember tfalse as tu.
   has_type_cases (induction Htyp) Case;
@@ -1220,10 +1224,10 @@ Proof with eauto.
 Qed.
 
 Lemma typing_inversion_if : forall Gamma t1 t2 t3 T,
-  has_type Gamma (tif t1 t2 t3) T ->
-  has_type Gamma t1 TBool 
-  /\ has_type Gamma t2 T
-  /\ has_type Gamma t3 T.
+  Gamma |- (tif t1 t2 t3) \in T ->
+  Gamma |- t1 \in TBool 
+  /\ Gamma |- t2 \in T
+  /\ Gamma |- t3 \in T.
 Proof with eauto.
   intros Gamma t1 t2 t3 T Hty.
   remember (tif t1 t2 t3) as t.
@@ -1236,8 +1240,8 @@ Proof with eauto.
 Qed.
 
 Lemma typing_inversion_unit : forall Gamma T,
-  has_type Gamma tunit T ->
-    subtype TUnit T.
+  Gamma |- tunit \in T ->
+    TUnit <: T.
 Proof with eauto.
   intros Gamma T Htyp. remember tunit as tu.
   has_type_cases (induction Htyp) Case;
@@ -1250,9 +1254,9 @@ Qed.
     us exactly what we'll actually require below. *)
 
 Lemma abs_arrow : forall x S1 s2 T1 T2, 
-  has_type empty (tabs x S1 s2) (TArrow T1 T2) ->
-     subtype T1 S1 
-  /\ has_type (extend empty x S1) s2 T2.
+  empty |- (tabs x S1 s2) \in (TArrow T1 T2) ->
+     T1 <: S1 
+  /\ (extend empty x S1) |- s2 \in T2.
 Proof with eauto.
   intros x S1 s2 T1 T2 Hty.
   apply typing_inversion_abs in Hty.
@@ -1292,9 +1296,9 @@ Inductive appears_free_in : id -> tm -> Prop :=
 Hint Constructors appears_free_in.
 
 Lemma context_invariance : forall Gamma Gamma' t S,
-     has_type Gamma t S  ->
+     Gamma |- t \in S  ->
      (forall x, appears_free_in x t -> Gamma x = Gamma' x)  ->
-     has_type Gamma' t S.
+     Gamma' |- t \in S.
 Proof with eauto.
   intros. generalize dependent Gamma'.
   has_type_cases (induction H) Case; 
@@ -1303,10 +1307,7 @@ Proof with eauto.
     apply T_Var... rewrite <- Heqv...
   Case "T_Abs".
     apply T_Abs... apply IHhas_type. intros x0 Hafi.
-    unfold extend. remember (beq_id x x0) as e.
-    destruct e...
-  Case "T_App".
-    apply T_App with T1...
+    unfold extend. destruct (eq_id_dec x x0)...
   Case "T_If".
     apply T_If...
 
@@ -1314,7 +1315,7 @@ Qed.
 
 Lemma free_in_context : forall x t T Gamma,
    appears_free_in x t ->
-   has_type Gamma t T ->
+   Gamma |- t \in T ->
    exists T', Gamma x = Some T'.
 Proof with eauto.
   intros x t T Gamma Hafi Htyp.
@@ -1322,8 +1323,7 @@ Proof with eauto.
       subst; inversion Hafi; subst...
   Case "T_Abs".
     destruct (IHHtyp H4) as [T Hctx]. exists T.
-    unfold extend in Hctx. apply not_eq_beq_id_false in H2. 
-    rewrite H2 in Hctx...  Qed.
+    unfold extend in Hctx. rewrite neq_id in Hctx...  Qed.
 
 (* ########################################## *)
 (** ** Substitution *)
@@ -1336,9 +1336,9 @@ Proof with eauto.
     well-typedness of subterms. *)
 
 Lemma substitution_preserves_typing : forall Gamma x U v t S,
-     has_type (extend Gamma x U) t S  ->
-     has_type empty v U   ->
-     has_type Gamma ([x:=v]t) S.
+     (extend Gamma x U) |- t \in S  ->
+     empty |- v \in U   ->
+     Gamma |- ([x:=v]t) \in S.
 Proof with eauto.
   intros Gamma x U v t S Htypt Htypv.
   generalize dependent S. generalize dependent Gamma.
@@ -1348,9 +1348,9 @@ Proof with eauto.
     destruct (typing_inversion_var _ _ _ Htypt) 
         as [T [Hctx Hsub]].
     unfold extend in Hctx.
-    remember (beq_id x y) as e. destruct e...
+    destruct (eq_id_dec x y)...
     SCase "x=y".
-      apply beq_id_eq in Heqe. subst.
+      subst.
       inversion Hctx; subst. clear Hctx.
       apply context_invariance with empty...
       intros x Hcontra.
@@ -1366,34 +1366,33 @@ Proof with eauto.
     destruct (typing_inversion_abs _ _ _ _ _ Htypt) 
       as [T2 [Hsub Htypt2]].
     apply T_Sub with (TArrow T1 T2)... apply T_Abs...
-    remember (beq_id x y) as e. destruct e.
+    destruct (eq_id_dec x y).
     SCase "x=y".
       eapply context_invariance...
-      apply beq_id_eq in Heqe. subst.
+      subst.
       intros x Hafi. unfold extend.
-      destruct (beq_id y x)...
+      destruct (eq_id_dec y x)...
     SCase "x<>y".
       apply IHt. eapply context_invariance...
       intros z Hafi. unfold extend.
-      remember (beq_id y z) as e0. destruct e0...
-      apply beq_id_eq in Heqe0. subst.
-      rewrite <- Heqe...
+      destruct (eq_id_dec y z)...
+      subst. rewrite neq_id... 
   Case "ttrue".
-      assert (subtype TBool S) 
+      assert (TBool <: S) 
         by apply (typing_inversion_true _ _  Htypt)...
   Case "tfalse".
-      assert (subtype TBool S) 
+      assert (TBool <: S) 
         by apply (typing_inversion_false _ _  Htypt)...
   Case "tif".
-    assert (has_type (extend Gamma x U) t1 TBool 
-            /\ has_type (extend Gamma x U) t2 S
-            /\ has_type (extend Gamma x U) t3 S) 
+    assert ((extend Gamma x U) |- t1 \in TBool 
+            /\ (extend Gamma x U) |- t2 \in S
+            /\ (extend Gamma x U) |- t3 \in S) 
       by apply (typing_inversion_if _ _ _ _ _ Htypt).
     inversion H as [H1 [H2 H3]].
     apply IHt1 in H1. apply IHt2 in H2. apply IHt3 in H3.
     auto.
   Case "tunit".
-    assert (subtype TUnit S) 
+    assert (TUnit <: S) 
       by apply (typing_inversion_unit _ _  Htypt)...
 Qed.
 
@@ -1410,19 +1409,20 @@ Qed.
     T].
 
     _Proof_: Let [t] and [T] be given such that [empty |- t : T].  We
-    go by induction on the structure of this typing derivation,
+    proceed by induction on the structure of this typing derivation,
     leaving [t'] general.  The cases [T_Abs], [T_Unit], [T_True], and
     [T_False] cases are vacuous because abstractions and constants
     don't step.  Case [T_Var] is vacuous as well, since the context is
     empty.
 
      - If the final step of the derivation is by [T_App], then there
-       are terms [t1] [t2] and types [T1] [T2] such that [t = t1 t2],
-       [T = T2], [empty |- t1 : T1 -> T2] and [empty |- t2 : T1].
+       are terms [t1] and [t2] and types [T1] and [T2] such that 
+       [t = t1 t2], [T = T2], [empty |- t1 : T1 -> T2], and 
+       [empty |- t2 : T1].
 
-       By inspection of the definition of the step relation, there are
-       three ways [t1 t2] can step.  Cases [ST_App1] and [ST_App2]
-       follow immediately by the induction hypotheses for the typing
+       By the definition of the step relation, there are three ways
+       [t1 t2] can step.  Cases [ST_App1] and [ST_App2] follow
+       immediately by the induction hypotheses for the typing
        subderivations and a use of [T_App].
 
        Suppose instead [t1 t2] steps by [ST_AppAbs].  Then [t1 =
@@ -1456,9 +1456,9 @@ Qed.
        subderivation and an application of [T_Sub].  [] *)
 
 Theorem preservation : forall t t' T,
-     has_type empty t T  ->
+     empty |- t \in T  ->
      t ==> t'  ->
-     has_type empty t' T.
+     empty |- t' \in T.
 Proof with eauto.
   intros t t' T HT.
   remember empty as Gamma. generalize dependent HeqGamma.
@@ -1502,7 +1502,7 @@ Qed.
 (* ###################################################### *)
 (** ** Exercises *)
 
-(** **** Exercise: 2 stars (variations) *)
+(** **** Exercise: 2 stars (variations)  *)
 (** Each part of this problem suggests a different way of
     changing the definition of the STLC with Unit and
     subtyping.  (These changes are not cumulative: each part
@@ -1543,13 +1543,12 @@ Qed.
                           -----------------------                    (S_Arrow')
                                S1->S2 <: T1->T2
 
-[]
-*) 
+[] *) 
 
 (* ###################################################################### *)
 (** * Exercise: Adding Products *)
 
-(** **** Exercise: 4 stars, optional (products) *)
+(** **** Exercise: 4 stars (products)  *)
 (** Adding pairs, projections, and product types to the system we have
     defined is a relatively straightforward matter.  Carry out this
     extension:
@@ -1558,21 +1557,26 @@ Qed.
       product types to the definitions of [ty] and [tm].  (Don't
       forget to add corresponding cases to [T_cases] and [t_cases].)
 
-    - Extend the well-formedness relation in the obvious way.
+    - Extend the substitution function and value relation as in 
+      MoreSTLC.
 
     - Extend the operational semantics with the same reduction rules
-      as in the last chapter.
+      as in MoreSTLC.
 
     - Extend the subtyping relation with this rule:
+
                         S1 <: T1     S2 <: T2
                         ---------------------                     (Sub_Prod)
                           S1 * S2 <: T1 * T2
+
     - Extend the typing relation with the same rules for pairs and
-      projections as in the last chapter.
+      projections as in MoreSTLC.
 
     - Extend the proofs of progress, preservation, and all their
       supporting lemmas to deal with the new constructs.  (You'll also
-      need to add some completely new lemmas.)  []
-*)
+      need to add some completely new lemmas.)  
+[] *)
 
+
+(** $Date: 2014-12-31 11:17:56 -0500 (Wed, 31 Dec 2014) $ *)
 
